compiler/scheme/proofs/scheme_to_cakeProofScript.sml
@@ -21,206 +21,62 @@ val _ = new_theory "scheme_to_cakeProof";
 
 val _ = (max_print_depth := 30);
 
-Theorem scheme_env1_def[allow_rebind, compute] = EVAL_RULE $ zDefine ‘
-  scheme_env1 = case evaluate_decs
-      (<|clock:=999;next_type_stamp:=0;next_exn_stamp:=0|> :num state)
-      <|v:=nsEmpty;c:=nsEmpty|>
-      (prim_types_program ++ [Dtype unknown_loc [(["'a"],"option",
-            [("None",[]); ("Some",[Atvar "'a"])])]] ++ [scheme_basis1]) of
-    | (st', Rval env) => env
-    | _ => <|v:=nsEmpty;c:=nsEmpty|>
-’;
-
-Definition cconses_def[simp]:
-  cconses = ["SNum"; "SBool"; "True"; "False";
-    "Prim";"SAdd";"SMul";"SMinus";"SEqv";"CallCC";
-    "[]"; "::"; "Some"; "None"; "Ex"; "Proc"; "Throw";"SList";"Wrong"]
+Definition closure_in_env_def:
+  closure_in_env env dec env_cl =
+    case dec of
+      | Dlet _ (Pvar x) e => nsLookup env.v (Short x) = SOME (case evaluate
+          (<|clock:=0;next_type_stamp:=0;next_exn_stamp:=0|> :num state)
+          env_cl [e] of
+        | (st', Rval [v]) => v)
+      | Dletrec _ funs => EVERY
+          (λ(f,_,_). nsLookup env.v (Short f) = SOME $ Recclosure env_cl funs f)
+        funs
 End
 
-Theorem scheme_env1_rw[simp] = SRULE [nsLookup_def] $ SIMP_CONV pure_ss [
-  SimpRHS, scheme_env1_def,
-  EVERY_DEF, cconses_def, MAP
-] “
-  EVERY (λ x . nsLookup scheme_env1.c x = nsLookup scheme_env1.c x) $
-    MAP Short cconses
-”;
-
-Theorem scheme_env2_def[allow_rebind, compute] = SRULE [] $
-  RESTR_EVAL_RULE [“scheme_env1”] $ zDefine ‘
-    scheme_env2 = case evaluate_decs
-        (<|clock:=999;next_type_stamp:=0;next_exn_stamp:=0|> :num state)
-        scheme_env1
-        [scheme_basis2] of
-      | (st', Rval env) => <|c:=scheme_env1.c;v:=nsAppend env.v scheme_env1.v|>
-      | _ => <|v:=nsEmpty;c:=nsEmpty|>
+Theorem scheme_cons_env_def[allow_rebind, compute] = EVAL_RULE $ zDefine ‘
+  scheme_cons_env = (case evaluate_decs
+               (<|clock:=0;next_type_stamp:=0;next_exn_stamp:=0|> :num state)
+               <|v:=nsEmpty;c:=nsEmpty|>
+               (prim_types_program ++ [Dtype unknown_loc [(["'a"],"option",
+                     [("None",[]); ("Some",[Atvar "'a"])])]] ++ [scheme_basis_types]) of
+             | (st', Rval env) => env).c
 ’;
 
-Theorem scheme_env2_rw[simp] = SRULE [GSYM CONJ_ASSOC] $
-CONJ (SRULE [Once scheme_env2_def] $ SCONV [] “
-  EVERY (λ x . nsLookup scheme_env2.c x = nsLookup scheme_env1.c x) $
-    MAP Short cconses
-”) $ SRULE [GSYM scheme_env1_def] $ EVAL “nsLookup scheme_env2.v (Short "sadd")”;
-
-Theorem scheme_env3_def[allow_rebind, compute] = SRULE [] $
-  RESTR_EVAL_RULE [“scheme_env2”] $ zDefine ‘
-    scheme_env3 = case evaluate_decs
-        (<|clock:=999;next_type_stamp:=0;next_exn_stamp:=0|> :num state)
-        scheme_env2
-        [scheme_basis3] of
-      | (st', Rval env) => <|c:=scheme_env2.c;v:=nsAppend env.v scheme_env2.v|>
-      | _ => <|v:=nsEmpty;c:=nsEmpty|>
+Theorem scheme_env_app_def[allow_rebind, compute] = EVAL_RULE $ zDefine ‘
+  scheme_env_app env <=>
+    env.c = scheme_cons_env ∧
+    EVERY (λ dec. ∃ env_cl . env_cl.c = scheme_cons_env ∧ closure_in_env env dec env_cl) scheme_basis
 ’;
 
-Theorem scheme_env3_rw[simp] = SRULE [GSYM CONJ_ASSOC] $
-CONJ (SRULE [Once scheme_env3_def] $ SCONV [] “
-  EVERY (λ x . nsLookup scheme_env3.c x = nsLookup scheme_env1.c x) $
-    MAP Short cconses
-”) $ LIST_CONJ $ map
-  (SRULE [
-    GSYM $ EVAL “scheme_env1”,
-    GSYM $ EVAL “scheme_env2”
-  ] o EVAL) [
-  “nsLookup scheme_env3.v (Short "sadd")”,
-  “nsLookup scheme_env3.v (Short "smul")”
-];
-
-Theorem scheme_env4_def[allow_rebind, compute] = SRULE [] $
-  RESTR_EVAL_RULE [“scheme_env3”] $ zDefine ‘
-    scheme_env4 = case evaluate_decs
-        (<|clock:=999;next_type_stamp:=0;next_exn_stamp:=0|> :num state)
-        scheme_env3
-        [scheme_basis4] of
-      | (st', Rval env) => <|c:=scheme_env3.c;v:=nsAppend env.v scheme_env3.v|>
-      | _ => <|v:=nsEmpty;c:=nsEmpty|>
+Theorem scheme_env_def[allow_rebind, compute] = RESTR_EVAL_RULE [``scheme_env_app``] $ zDefine ‘
+  scheme_env env <=>
+    env.c = scheme_cons_env ∧
+    ∃ env_app .
+      scheme_env_app env_app ∧
+      closure_in_env env scheme_basis_app env_app
 ’;
-
-Theorem scheme_env4_rw[simp] = SRULE [GSYM CONJ_ASSOC] $
-CONJ (SRULE [Once scheme_env4_def] $ SCONV [] “
-  EVERY (λ x . nsLookup scheme_env4.c x = nsLookup scheme_env1.c x) $
-    MAP Short cconses
-”) $ LIST_CONJ $ map
-  (SRULE [
-    GSYM $ EVAL “scheme_env1”,
-    GSYM $ EVAL “scheme_env2”,
-    GSYM $ EVAL “scheme_env3”
-  ] o EVAL) [
-  “nsLookup scheme_env4.v (Short "sadd")”,
-  “nsLookup scheme_env4.v (Short "smul")”,
-  “nsLookup scheme_env4.v (Short "sminus")”
-];
-
-Theorem scheme_env5_def[allow_rebind, compute] = SRULE [] $
-  RESTR_EVAL_RULE [“scheme_env4”] $ zDefine ‘
-    scheme_env5 = case evaluate_decs
-        (<|clock:=999;next_type_stamp:=0;next_exn_stamp:=0|> :num state)
-        scheme_env4
-        [scheme_basis5] of
-      | (st', Rval env) => <|c:=scheme_env4.c;v:=nsAppend env.v scheme_env4.v|>
-      | _ => <|v:=nsEmpty;c:=nsEmpty|>
-’;
-
-Theorem scheme_env5_rw[simp] = SRULE [GSYM CONJ_ASSOC] $
-CONJ (SRULE [Once scheme_env5_def] $ SCONV [] “
-  EVERY (λ x . nsLookup scheme_env5.c x = nsLookup scheme_env1.c x) $
-    MAP Short cconses
-”) $ LIST_CONJ $ map
-  (SRULE [
-    GSYM $ EVAL “scheme_env1”,
-    GSYM $ EVAL “scheme_env2”,
-    GSYM $ EVAL “scheme_env3”,
-    GSYM $ EVAL “scheme_env4”
-  ] o EVAL) [
-  “nsLookup scheme_env5.v (Short "sadd")”,
-  “nsLookup scheme_env5.v (Short "smul")”,
-  “nsLookup scheme_env5.v (Short "sminus")”,
-  “nsLookup scheme_env5.v (Short "seqv")”
-];
-
-Theorem scheme_env6_def[allow_rebind, compute] = SRULE [] $
-  RESTR_EVAL_RULE [“scheme_env5”] $ zDefine ‘
-    scheme_env6 = case evaluate_decs
-        (<|clock:=999;next_type_stamp:=0;next_exn_stamp:=0|> :num state)
-        scheme_env5
-        [scheme_basis6] of
-      | (st', Rval env) => <|c:=scheme_env5.c;v:=nsAppend env.v scheme_env5.v|>
-      | _ => <|v:=nsEmpty;c:=nsEmpty|>
-’;
-
-Theorem scheme_env6_rw[simp] = SRULE [GSYM CONJ_ASSOC] $
-CONJ (SRULE [Once scheme_env6_def] $ SCONV [] “
-  EVERY (λ x . nsLookup scheme_env6.c x = nsLookup scheme_env1.c x) $
-    MAP Short cconses
-”) $ LIST_CONJ $ map
-  (SRULE [
-    GSYM $ EVAL “scheme_env1”,
-    GSYM $ EVAL “scheme_env2”,
-    GSYM $ EVAL “scheme_env3”,
-    GSYM $ EVAL “scheme_env4”,
-    GSYM $ EVAL “scheme_env5”
-  ] o EVAL) [
-  “nsLookup scheme_env6.v (Short "sadd")”,
-  “nsLookup scheme_env6.v (Short "smul")”,
-  “nsLookup scheme_env6.v (Short "sminus")”,
-  “nsLookup scheme_env6.v (Short "seqv")”,
-  “nsLookup scheme_env6.v (Short "throw")”
-];
-
-Theorem scheme_env7_def[allow_rebind, compute] = SRULE [] $
-  RESTR_EVAL_RULE [“scheme_env6”] $ zDefine ‘
-    scheme_env7 = case evaluate_decs
-        (<|clock:=999;next_type_stamp:=0;next_exn_stamp:=0|> :num state)
-        scheme_env6
-        [scheme_basis7] of
-      | (st', Rval env) => <|c:=scheme_env6.c;v:=nsAppend env.v scheme_env6.v|>
-      | _ => <|v:=nsEmpty;c:=nsEmpty|>
-’;
-
-Theorem scheme_env7_rw[simp] = SRULE [GSYM CONJ_ASSOC] $
-CONJ (SRULE [Once scheme_env7_def] $ SCONV [] “
-  EVERY (λ x . nsLookup scheme_env7.c x = nsLookup scheme_env1.c x) $
-    MAP Short cconses
-”) $ LIST_CONJ $ map
-  (SRULE [
-    GSYM $ EVAL “scheme_env1”,
-    GSYM $ EVAL “scheme_env2”,
-    GSYM $ EVAL “scheme_env3”,
-    GSYM $ EVAL “scheme_env4”,
-    GSYM $ EVAL “scheme_env5”,
-    GSYM $ EVAL “scheme_env6”
-  ] o EVAL) [
-  “nsLookup scheme_env7.v (Short "sadd")”,
-  “nsLookup scheme_env7.v (Short "smul")”,
-  “nsLookup scheme_env7.v (Short "sminus")”,
-  “nsLookup scheme_env7.v (Short "seqv")”,
-  “nsLookup scheme_env7.v (Short "throw")”,
-  “nsLookup scheme_env7.v (Short "callcc")”,
-  “nsLookup scheme_env7.v (Short "app")”
-];
 
 Theorem scheme_env'_def[allow_rebind, compute] = EVAL_RULE $ zDefine ‘
-  scheme_env' = case evaluate_decs (<|clock:=999;next_type_stamp:=0;next_exn_stamp:=0|> :num state) <|v:=nsEmpty;c:=nsEmpty|> (prim_types_program ++ [Dtype unknown_loc [(["'a"],"option",
-            [("None",[]); ("Some",[Atvar "'a"])])]] ++ scheme_basis) of
-    | (st', Rval env) => env
-    | _ => <|v:=nsEmpty;c:=nsEmpty|>
+  scheme_env' = case evaluate_decs (<|clock:=999;next_type_stamp:=0;next_exn_stamp:=0|> :num state)
+                  <|v:=nsEmpty;c:=nsEmpty|>
+                  (prim_types_program ++ [Dtype unknown_loc [(["'a"],"option", [("None",[]); ("Some",[Atvar "'a"])])]]
+                    ++ [scheme_basis_types] ++ scheme_basis ++ [scheme_basis_app]) of
+                | (st', Rval env) => env
 ’;
 
-Definition vconses_def[simp]:
-  vconses = ["sadd"; "smul"; "sminus"; "seqv"; "throw"; "callcc"; "app"]
-End
-
-Theorem scheme_env_def[allow_rebind, compute] = SRULE [GSYM CONJ_ASSOC] $ zDefine ‘
-  scheme_env env
-  ⇔
-  EVERY (λ x . nsLookup env.c x = nsLookup scheme_env7.c x) $
-    MAP Short cconses ∧
-  EVERY (λ x . nsLookup env.v x = nsLookup scheme_env7.v x) $
-    MAP Short vconses
-’
-
 Theorem basis_scheme_env:
-    scheme_env scheme_env'
+  scheme_env scheme_env'
 Proof
-  EVAL_TAC
+  simp[scheme_env_def, PULL_EXISTS]
+  >> qexists ‘case evaluate_decs (<|clock:=999;next_type_stamp:=0;next_exn_stamp:=0|> :num state)
+                <|v:=nsEmpty;c:=nsEmpty|>
+                (prim_types_program ++ [Dtype unknown_loc [(["'a"],"option", [("None",[]); ("Some",[Atvar "'a"])])]]
+                  ++ [scheme_basis_types] ++ scheme_basis) of
+              | (st', Rval env) => env’
+  >> EVAL_TAC
+  >> rpt strip_tac
+  >> irule_at (Pos last) EQ_REFL
+  >> simp[]
 QED
 
 (*
@@ -241,20 +97,168 @@ before and after step in CEK machine
         | _ => (\k2 -> k2 (SNum 2)) (\t -> t)))
 *)
 
+Theorem scheme_conses_def[allow_rebind, compute] = EVAL_RULE $ zDefine‘
+  scheme_conses = case scheme_cons_env of
+    Bind cs _ => MAP FST cs
+’;
+
+Theorem scheme_runtime_funs_def[allow_rebind, compute] = EVAL_RULE $ zDefine‘
+  scheme_runtime_funs = FOLDL (λ acc dec. acc ++ case dec of
+    | Dlet _ (Pvar x) _ => [x]
+    | Dletrec _ funs => MAP FST funs) [] $
+    scheme_basis ++ [scheme_basis_app]
+’;
+
 Definition scheme_typestamp_def:
-  scheme_typestamp con = SND $ THE $ nsLookup scheme_env1.c (Short con)
+  scheme_typestamp con = SND $ THE $ nsLookup scheme_cons_env (Short con)
 End
 
-Theorem scheme_typestamp_def[allow_rebind, simp] = SRULE [] $
-  SIMP_CONV pure_ss [SimpRHS, scheme_typestamp_def, EVERY_DEF, cconses_def]
-  “EVERY (λ x . scheme_typestamp x = scheme_typestamp x) cconses”;
+Theorem scheme_typestamp_def[allow_rebind, simp, compute] = SRULE [] $
+  SIMP_CONV pure_ss [SimpRHS, scheme_typestamp_def, EVERY_DEF,
+      scheme_conses_def, SND, THE_DEF, nsLookup_def, scheme_cons_env_def]
+    “EVERY (λ x . scheme_typestamp x = scheme_typestamp x) scheme_conses”;
+
+Definition muts_loc_def:
+  muts_loc nl [] l = nl + l /\
+  muts_loc nl (Refv _::refs) 0 = nl /\
+  muts_loc nl (Refv _::refs) (SUC l) = muts_loc (SUC nl) refs l /\
+  muts_loc nl (_::refs) l = muts_loc (SUC nl) refs l
+End
+
+Theorem muts_loc_props:
+  ! nl refs l . muts_loc nl refs l >= nl + l /\ muts_loc (SUC nl) refs l = SUC (muts_loc nl refs l)
+Proof
+  ho_match_mp_tac muts_loc_ind
+  >> simp[muts_loc_def]
+QED
+
+Theorem muts_loc_mono = cj 1 muts_loc_props;
+Theorem muts_loc_SUC[simp] = cj 2 muts_loc_props;
+
+Theorem muts_loc_FILTER:
+  ! refs l .
+    (muts_loc 0 refs l < LENGTH refs
+     <=> l < LENGTH (FILTER (\ref. case ref of | Refv _ => T | _ => F) refs))
+    /\
+    EL (muts_loc 0 refs l) refs
+     = EL l $ FILTER (\ref. case ref of | Refv _ => T | _ => F) refs
+Proof
+  Induct >> Induct
+  >> simp[muts_loc_def]
+  >> gen_tac >> Cases
+  >> simp[muts_loc_def]
+QED
+
+Theorem muts_loc_alloc_same:
+  ! refs l mlv .
+    muts_loc 0 refs l = muts_loc 0 (refs ++ [Refv mlv]) l
+Proof
+  Induct >> Induct
+  >> simp[muts_loc_def]
+  >> gen_tac >> Cases
+  >> simp[muts_loc_def]
+QED
+
+Theorem muts_loc_LUPDATE_same:
+  ! refs l l' mlv mlv' .
+    EL l' refs = Refv mlv
+    ==>
+    muts_loc 0 refs l = muts_loc 0 (LUPDATE (Refv mlv') l' refs) l
+Proof
+  Induct >> Induct
+  >> simp[muts_loc_def, LUPDATE_def] >- (
+    gen_tac >> Cases >> Cases
+    >> simp[muts_loc_def, LUPDATE_def]
+  )
+  >> gen_tac >> gen_tac >> Cases
+  >> simp[muts_loc_def, LUPDATE_def]
+QED
+
+Definition pairs_loc_def:
+  pairs_loc nl [] l = nl + l /\
+  pairs_loc nl (Varray _::refs) 0 = nl /\
+  pairs_loc nl (Varray _::refs) (SUC l) = pairs_loc (SUC nl) refs l /\
+  pairs_loc nl (_::refs) l = pairs_loc (SUC nl) refs l
+End
+
+Theorem pairs_loc_props:
+  ! nl refs l . pairs_loc nl refs l >= nl + l /\ pairs_loc (SUC nl) refs l = SUC (pairs_loc nl refs l)
+Proof
+  ho_match_mp_tac pairs_loc_ind
+  >> simp[pairs_loc_def]
+QED
+
+Theorem pairs_loc_mono = cj 1 pairs_loc_props;
+Theorem pairs_loc_SUC[simp] = cj 2 pairs_loc_props;
+
+Theorem pairs_loc_FILTER:
+  ! refs l .
+    (pairs_loc 0 refs l < LENGTH refs
+     <=> l < LENGTH (FILTER (\ref. case ref of | Varray _ => T | _ => F) refs))
+    /\
+    EL (pairs_loc 0 refs l) refs
+     = EL l $ FILTER (\ref. case ref of | Varray _ => T | _ => F) refs
+Proof
+  Induct >> Induct
+  >> simp[pairs_loc_def]
+  >> gen_tac >> Cases
+  >> simp[pairs_loc_def]
+QED
+
+Theorem pairs_loc_alloc_diff:
+  ! refs l mlv .
+    pairs_loc 0 refs l < LENGTH refs ==> pairs_loc 0 refs l = pairs_loc 0 (refs ++ [Refv mlv]) l
+Proof
+  Induct >> Induct
+  >> simp[pairs_loc_def]
+  >> gen_tac >> Cases
+  >> simp[pairs_loc_def]
+QED
+
+Theorem pairs_loc_LUPDATE_diff:
+  ! refs l l' mlv mlv' .
+    EL l' refs = Refv mlv
+    ==>
+    pairs_loc 0 refs l = pairs_loc 0 (LUPDATE (Refv mlv') l' refs) l
+Proof
+  Induct >> Induct
+  >> simp[pairs_loc_def, LUPDATE_def]
+  >> gen_tac >> Cases >> Cases
+  >> simp[pairs_loc_def, LUPDATE_def]
+QED
 
 Inductive env_rel:
   FEVERY (λ (x, n).
-    nsLookup env.v (Short ("var" ++ explode x)) = SOME (Loc T n)) se
+    nsLookup env.v (Short ("var" ++ explode x)) = SOME (Loc T (muts_loc 0 refs n))) se
   ⇒
-  env_rel se env
+  env_rel refs se env
 End
+
+Theorem env_rel_alloc:
+  ! refs mlv se env .
+    env_rel refs se env ==> env_rel (refs ++ [Refv mlv]) se env
+Proof
+  simp[env_rel_cases]
+  >> rpt strip_tac
+  >> irule FEVERY_MONO
+  >> pop_assum $ irule_at $ Pos last
+  >> PairCases
+  >> simp[muts_loc_alloc_same]
+QED
+
+Theorem env_rel_LUPDATE_same:
+  ! refs l mlv'1 mlv'2 se env .
+    EL l refs = Refv mlv'1
+    ==>
+    env_rel refs se env ==> env_rel (LUPDATE (Refv mlv'2) l refs) se env
+Proof
+  simp[env_rel_cases]
+  >> rpt strip_tac
+  >> irule FEVERY_MONO
+  >> pop_assum $ irule_at $ Pos last
+  >> PairCases
+  >> rw[muts_loc_LUPDATE_same]
+QED
 
 Theorem vcons_list_def[allow_rebind] = SRULE [] $ Define ‘
   vcons_list [] = Conv (SOME (scheme_typestamp "[]")) [] ∧
@@ -272,145 +276,423 @@ End
 
 Inductive val_cont_rels:
 [~SBool_T:]
-  ml_v_vals' (SBool T) $
+  ml_v_vals refs (SBool T) $
     Conv (SOME (scheme_typestamp "SBool")) [Conv (SOME (scheme_typestamp "True")) []]
 [~SBool_F:]
-  ml_v_vals' (SBool F) $
+  ml_v_vals refs (SBool F) $
     Conv (SOME (scheme_typestamp "SBool")) [Conv (SOME (scheme_typestamp "False")) []]
 [~SNum:]
-  ml_v_vals' (SNum i) $
+  ml_v_vals refs (SNum i) $
     Conv (SOME (scheme_typestamp "SNum")) [Litv (IntLit i)]
 [~Prim_SAdd:]
-  ml_v_vals' (Prim SAdd) $
+  ml_v_vals refs (Prim SAdd) $
     Conv (SOME (scheme_typestamp "Prim")) [Conv (SOME (scheme_typestamp "SAdd")) []]
 [~Prim_SMul:]
-  ml_v_vals' (Prim SMul) $
+  ml_v_vals refs (Prim SMul) $
     Conv (SOME (scheme_typestamp "Prim")) [Conv (SOME (scheme_typestamp "SMul")) []]
 [~Prim_SMinus:]
-  ml_v_vals' (Prim SMinus) $
+  ml_v_vals refs (Prim SMinus) $
     Conv (SOME (scheme_typestamp "Prim")) [Conv (SOME (scheme_typestamp "SMinus")) []]
 [~Prim_SEqv:]
-  ml_v_vals' (Prim SEqv) $
+  ml_v_vals refs (Prim SEqv) $
     Conv (SOME (scheme_typestamp "Prim")) [Conv (SOME (scheme_typestamp "SEqv")) []]
 [~Prim_CallCC:]
-  ml_v_vals' (Prim CallCC) $
+  ml_v_vals refs (Prim CallCC) $
     Conv (SOME (scheme_typestamp "Prim")) [Conv (SOME (scheme_typestamp "CallCC")) []]
+[~Prim_Cons:]
+  ml_v_vals refs (Prim Cons) $
+    Conv (SOME (scheme_typestamp "Prim")) [Conv (SOME (scheme_typestamp "Cons")) []]
+[~Prim_Car:]
+  ml_v_vals refs (Prim Car) $
+    Conv (SOME (scheme_typestamp "Prim")) [Conv (SOME (scheme_typestamp "Car")) []]
+[~Prim_Cdr:]
+  ml_v_vals refs (Prim Cdr) $
+    Conv (SOME (scheme_typestamp "Prim")) [Conv (SOME (scheme_typestamp "Cdr")) []]
 [~Prim_Wrong:]
-  ml_v_vals' (Wrong s) $
+  ml_v_vals refs (Wrong s) $
     Conv (SOME (scheme_typestamp "Wrong")) [Litv (StrLit s)]
 [~Proc:]
   scheme_env env ∧
-  env_rel se env ∧
+  env_rel refs se env ∧
   ce = cps_transform e ∧
   inner = proc_ml xs xp "k" ce
   ⇒
-  ml_v_vals' (Proc se xs xp e) $
+  ml_v_vals refs (Proc se xs xp e) $
     Conv (SOME (scheme_typestamp "Proc")) [
       Closure env "k" $ Fun "ts" inner
     ]
 [~Throw:]
-  cont_rel ks kv
+  cont_rel refs ks kv
   ⇒
-  ml_v_vals' (Throw ks) $
+  ml_v_vals refs (Throw ks) $
     Conv (SOME (scheme_typestamp "Throw")) [kv]
 [~SList:]
-  LIST_REL ml_v_vals' vs mlvs
+  LIST_REL (ml_v_vals refs) vs mlvs
   ⇒
-  ml_v_vals' (SList vs) $
+  ml_v_vals refs (SList vs) $
     Conv (SOME (scheme_typestamp "SList")) [vcons_list mlvs]
+[~PairP:]
+  pairs_loc 0 refs l < LENGTH refs
+  ⇒
+  ml_v_vals refs (PairP l) $
+    Conv (SOME (scheme_typestamp "PairP")) [Loc T (pairs_loc 0 refs l)]
+[~Nul:]
+  ml_v_vals refs Null $
+    Conv (SOME (scheme_typestamp "Null")) []
 
 [~Id:]
   scheme_env env
   ⇒
-  cont_rel []
+  cont_rel refs []
     (Closure env "t" (Var (Short "t")))
 [~CondK:]
-  cont_rel ks kv ∧
+  cont_rel refs ks kv ∧
   nsLookup env.v (Short "k") = SOME kv ∧
   ct = cps_transform te ∧
   cf = cps_transform fe ∧
   scheme_env env ∧
-  env_rel se env
+  env_rel refs se env
   ⇒
-  cont_rel ((se, CondK te fe) :: ks)
+  cont_rel refs ((se, CondK te fe) :: ks)
     (Closure env "t" $ Mat (Var (Short "t")) [
       (Pcon (SOME $ Short "SBool") [Pcon (SOME $ Short "False") []],
         App Opapp [cf; Var (Short "k")]);
       (Pany, App Opapp [ct;  Var (Short "k")])
     ])
 [~ApplyK_NONE:]
-  cont_rel ks kv ∧
+  cont_rel refs ks kv ∧
   nsLookup env.v (Short "k") = SOME kv ∧
   inner = cps_transform_app (Var (Short "t")) [] es (Var (Short "k")) ∧
   scheme_env env ∧
-  env_rel se env
+  env_rel refs se env
   ⇒
-  cont_rel ((se, ApplyK NONE es) :: ks)
+  cont_rel refs ((se, ApplyK NONE es) :: ks)
     (Closure env "t" $ inner)
 [~ApplyK_SOME:]
-  cont_rel ks kv ∧
+  cont_rel refs ks kv ∧
   nsLookup env.v (Short "k") = SOME kv ∧
   (t, ts) = cps_app_ts vs ∧
   inner = cps_transform_app (Var (Short "t"))
-    (Var (Short t) :: MAP (Var o Short) ts) es (Var (Short "k")) ∧
-  ml_v_vals' fn mlfn ∧
+    (MAP (Var o Short) (t::ts)) es (Var (Short "k")) ∧
+  ml_v_vals refs fn mlfn ∧
   nsLookup env.v (Short "t") = SOME mlfn ∧
-  LIST_REL ml_v_vals' vs mlvs ∧
+  LIST_REL (ml_v_vals refs) vs mlvs ∧
   LIST_REL (λ x mlv . nsLookup env.v (Short x) = SOME mlv) ts mlvs ∧
   scheme_env env ∧
-  env_rel se env
+  env_rel refs se env
   ⇒
-  cont_rel ((se, ApplyK (SOME (fn, vs)) es) :: ks)
+  cont_rel refs ((se, ApplyK (SOME (fn, vs)) es) :: ks)
     (Closure env t $ inner)
 [~BeginK:]
-  cont_rel ks kv ∧
+  cont_rel refs ks kv ∧
   nsLookup env.v (Short "k") = SOME kv ∧
   inner = cps_transform_seq (Var (Short "k")) es e ∧
   scheme_env env ∧
-  env_rel se env
+  env_rel refs se env
   ⇒
-  cont_rel ((se, BeginK es e) :: ks)
+  cont_rel refs ((se, BeginK es e) :: ks)
     (Closure env "_" $ inner)
 [~SetK:]
-  cont_rel ks kv ∧
+  cont_rel refs ks kv ∧
   nsLookup env.v (Short "k") = SOME kv ∧
   inner = refunc_set (Var (Short "t")) (Var (Short "k")) x ∧
   scheme_env env ∧
-  env_rel se env
+  env_rel refs se env
   ⇒
-  cont_rel ((se, SetK x) :: ks)
+  cont_rel refs ((se, SetK x) :: ks)
     (Closure env "t" $ inner)
 [~LetinitK:]
-  cont_rel ks kv ∧
+  cont_rel refs ks kv ∧
   nsLookup env.v (Short "k") = SOME kv ∧
   (t, ts) = cps_app_ts xvs ∧
   inner = cps_transform_letinit
     ((x,Var (Short t))::ZIP (MAP FST xvs, MAP (Var o Short) ts))
     bs e (Var (Short "k")) ∧
-  LIST_REL ml_v_vals' (MAP SND xvs) mlvs ∧
+  LIST_REL (ml_v_vals refs) (MAP SND xvs) mlvs ∧
   LIST_REL (λ x mlv . nsLookup env.v (Short x) = SOME mlv) ts mlvs ∧
   scheme_env env ∧
-  env_rel se env
+  env_rel refs se env
   ⇒
-  cont_rel ((se, LetinitK xvs x bs e) :: ks)
+  cont_rel refs ((se, LetinitK xvs x bs e) :: ks)
     (Closure env t $ inner)
 End
 
 Theorem val_cont_rels_ind[allow_rebind] = SRULE [] $ val_cont_rels_ind;
-Theorem ml_v_vals'_cases = SRULE [] $ cj 1 val_cont_rels_cases;
+Theorem ml_v_vals_cases = SRULE [] $ cj 1 val_cont_rels_cases;
 Theorem cont_rel_cases = cj 2 val_cont_rels_cases;
+
+Theorem val_cont_rel_mono:
+  ! refs mlv' .
+    (! v mlv . ml_v_vals refs v mlv ==> ml_v_vals (refs ++ [Refv mlv']) v mlv) /\
+    (! ks kv . cont_rel refs ks kv ==> cont_rel (refs ++ [Refv mlv']) ks kv)
+Proof
+  rpt gen_tac
+  >> ho_match_mp_tac val_cont_rels_ind
+  >> rpt strip_tac
+  >> simp[Once ml_v_vals_cases, env_rel_alloc]
+  >- (
+    irule_at (Pos hd) EQ_REFL >> gvs[SF ETA_ss]
+  )
+  >- (
+    simp[pairs_loc_alloc_diff]
+    >> simp[GSYM pairs_loc_alloc_diff]
+  )
+  >> simp[Once cont_rel_cases, env_rel_alloc]
+  >> irule_at (Pos hd) EQ_REFL
+  >> first_assum $ irule_at (Pos last)
+  >> gvs[SF ETA_ss]
+QED
+
+Theorem ml_v_vals_mono = SRULE [PULL_FORALL, AND_IMP_INTRO] $
+  cj 1 val_cont_rel_mono;
+Theorem cont_rel_mono = SRULE [PULL_FORALL, AND_IMP_INTRO] $
+  cj 2 val_cont_rel_mono;
+
+Theorem val_cont_rel_LUPDATE_same:
+  ! refs l mlv'1 mlv'2 .
+    EL l refs = Refv mlv'1
+    ==>
+    (! v mlv . ml_v_vals refs v mlv ==> ml_v_vals (LUPDATE (Refv mlv'2) l refs) v mlv) /\
+    (! ks kv . cont_rel refs ks kv ==> cont_rel (LUPDATE (Refv mlv'2) l refs) ks kv)
+Proof
+  rpt gen_tac >> strip_tac
+  >> ho_match_mp_tac val_cont_rels_ind
+  >> rpt strip_tac
+  >> simp[Once ml_v_vals_cases] >- simp[env_rel_LUPDATE_same]
+  >- (
+    irule_at (Pos hd) EQ_REFL >> gvs[SF ETA_ss]
+  )
+  >- (
+    simp[pairs_loc_LUPDATE_diff]
+    >> simp[GSYM pairs_loc_LUPDATE_diff]
+  )
+  >> simp[Once cont_rel_cases, env_rel_LUPDATE_same]
+  >> irule_at (Pos hd) EQ_REFL
+  >> first_assum $ irule_at (Pos last)
+  >> gvs[SF ETA_ss]
+QED
+
+Theorem ml_v_vals_LUPDATE_same = SRULE [PULL_FORALL, AND_IMP_INTRO] $
+  cj 1 val_cont_rel_LUPDATE_same;
+Theorem cont_rel_LUPDATE_same = SRULE [PULL_FORALL, AND_IMP_INTRO] $
+  cj 2 val_cont_rel_LUPDATE_same;
 
 val (store_entry_rel_rules,store_entry_rel_ind,store_entry_rel_cases) =
 (fn (x,y,z) => (SRULE [] x,SRULE [] y, SRULE [] z)) $ Hol_reln ‘
-  (ml_v_vals' v mlv
+  (ml_v_vals refs v mlv
   ⇒
-  store_entry_rel (SOME v) (Refv (Conv (SOME (scheme_typestamp "Some")) [mlv]))) ∧
-  store_entry_rel NONE (Refv (Conv (SOME (scheme_typestamp "None")) []))
+  store_entry_rel refs (SOME v) (Refv (Conv (SOME (scheme_typestamp "Some")) [mlv]))) ∧
+  store_entry_rel refs NONE (Refv (Conv (SOME (scheme_typestamp "None")) []))
 ’;
 
+Inductive pair_rel:
+  ml_v_vals refs v mlv ∧
+  ml_v_vals refs v' mlv'
+  ⇒
+  pair_rel refs (v, v') (Varray [mlv; mlv'])
+End
+
+Inductive muts_rel:
+[~empty:]
+  muts_rel refs' [] []
+[~mut:]
+  store_entry_rel refs' mut ref ∧
+  muts_rel refs' muts refs
+  ⇒
+  muts_rel refs' (mut::muts) (ref::refs)
+[~pair:]
+  muts_rel refs' muts refs
+  ⇒
+  muts_rel refs' muts (Varray vs::refs)
+End
+
+Inductive pairs_rel:
+[~empty:]
+  pairs_rel refs' [] []
+[~pair:]
+  pair_rel refs' pair ref ∧
+  pairs_rel refs' pairs refs
+  ⇒
+  pairs_rel refs' (pair::pairs) (ref::refs)
+[~mut:]
+  pairs_rel refs' pairs refs
+  ⇒
+  pairs_rel refs' pairs (Refv v::refs)
+End
+
+Definition store_rel_def[simp]:
+  store_rel st refs <=> muts_rel refs st.muts refs ∧ pairs_rel refs st.pairs refs
+End
+
+Theorem muts_rel_FILTER:
+  ! refs' muts refs .
+    muts_rel refs' muts refs
+    ==>
+    LIST_REL (store_entry_rel refs') muts $
+      FILTER (\ref. case ref of | Refv _ => T | _ => F) refs
+Proof
+  gen_tac >> ho_match_mp_tac muts_rel_ind
+  >> simp[]
+  >> rpt strip_tac
+  >> CASE_TAC
+  >> gvs[Once store_entry_rel_cases]
+  >> simp[Once store_entry_rel_cases]
+QED
+
+Theorem muts_rel_LUPDATE_same:
+  ! refs' muts refs .
+    muts_rel refs' muts refs
+    ==>
+    ! mut ref l .
+      store_entry_rel refs' mut ref
+      ==>
+      muts_rel refs' muts refs /\
+      muts_rel refs' (LUPDATE mut l muts) (LUPDATE ref (muts_loc 0 refs l) refs)
+Proof
+  gen_tac
+  >> ho_match_mp_tac muts_rel_ind
+  >> simp[LUPDATE_def]
+  >> simp[Once muts_rel_cases]
+  >> rpt strip_tac >- (
+    first_x_assum $ drule >> strip_tac
+    >> simp[Once muts_rel_cases]
+  )
+  >- (
+    gvs[Once store_entry_rel_cases]
+    >> Cases_on `l`
+    >> gvs[LUPDATE_def, muts_loc_def]
+    >> first_x_assum $ drule >> strip_tac
+    >> simp[Once muts_rel_cases]
+    >> simp[store_entry_rel_cases]
+  )
+  >- (
+    irule muts_rel_pair
+    >> last_x_assum drule >> strip_tac
+    >> simp[]
+  )
+  >> simp[muts_loc_def, LUPDATE_def, Once muts_rel_cases]
+QED
+
+Theorem muts_rel_LUPDATE_same[allow_rebind] = cj 2 muts_rel_LUPDATE_same;
+
+Theorem muts_rel_mono:
+  ! (refs'1:'a store_v list) (refs'2:'a store_v list) .
+    (! mut ref . store_entry_rel refs'1 mut ref ==> store_entry_rel refs'2 mut ref)
+    ==>
+    ! muts refs .
+      muts_rel refs'1 muts refs ==> muts_rel refs'2 muts refs
+Proof
+  rpt gen_tac >> strip_tac
+  >> ho_match_mp_tac muts_rel_ind
+  >> rpt strip_tac
+  >> gvs[store_entry_rel_cases]
+  >> simp[Once muts_rel_cases]
+  >> simp[store_entry_rel_cases]
+QED
+
+Theorem muts_rel_loc:
+  ! refs' muts refs l .
+    l < LENGTH muts /\ muts_rel refs' muts refs 
+    ==>
+    muts_loc 0 refs l < LENGTH refs /\
+    store_entry_rel refs' (EL l muts) (EL (muts_loc 0 refs l) refs)
+Proof
+  rpt strip_tac
+  >> dxrule_then assume_tac muts_rel_FILTER
+  >> gvs[LIST_REL_EL_EQN, muts_loc_FILTER]
+QED
+
+Theorem muts_rel_loc_alloc:
+  ! mlv muts refs .
+    muts_rel refs muts refs
+    ==>
+    muts_loc 0 refs (LENGTH muts) = LENGTH refs
+Proof
+  rpt strip_tac
+  >> dxrule_then assume_tac muts_rel_FILTER
+  >> dxrule_then assume_tac LIST_REL_LENGTH
+  >> simp[muts_loc_FILTER]
+QED
+
+Theorem pairs_rel_FILTER:
+  ! refs' pairs refs .
+    pairs_rel refs' pairs refs
+    ==>
+    LIST_REL (pair_rel refs') pairs $
+      FILTER (\ref. case ref of | Varray _ => T | _ => F) refs
+Proof
+  gen_tac >> ho_match_mp_tac pairs_rel_ind
+  >> simp[]
+  >> rpt strip_tac
+  >> CASE_TAC
+  >> gvs[Once pair_rel_cases]
+  >> simp[Once pair_rel_cases]
+QED
+
+Theorem pairs_rel_LUPDATE_diff:
+  ! refs' pairs refs .
+    pairs_rel refs' pairs refs
+    ==>
+    ! mut ref l .
+      store_entry_rel refs' mut ref
+      ==>
+      pairs_rel refs' pairs refs /\
+      pairs_rel refs' pairs (LUPDATE ref (muts_loc 0 refs l) refs)
+Proof
+  gen_tac
+  >> ho_match_mp_tac pairs_rel_ind
+  >> simp[LUPDATE_def]
+  >> simp[Once pairs_rel_cases]
+  >> rpt strip_tac
+  >> first_x_assum $ drule_then $ mp_tac o SRULE [Once $ GSYM PULL_FORALL]
+  >> strip_tac
+  >~ [`muts_loc 0 (Refv _::_) _`]
+  >- (
+    Cases_on `l`
+    >> simp[LUPDATE_def, muts_loc_def]
+    >> gvs[Once store_entry_rel_cases]
+    >> simp[Once pairs_rel_cases]
+    >> simp[Once pairs_rel_cases]
+  )
+  >> gvs[Once pair_rel_cases]
+  >> simp[LUPDATE_def, muts_loc_def]
+  >> simp[Once pairs_rel_cases]
+  >> simp[Once pair_rel_cases]
+QED
+
+Theorem pairs_rel_LUPDATE_diff[allow_rebind] = cj 2 pairs_rel_LUPDATE_diff;
+
+Theorem pairs_rel_mono:
+  ! (refs'1:'a store_v list) (refs'2:'a store_v list) .
+    (! pair ref . pair_rel refs'1 pair ref ==> pair_rel refs'2 pair ref)
+    ==>
+    ! pairs refs .
+      pairs_rel refs'1 pairs refs ==> pairs_rel refs'2 pairs refs
+Proof
+  rpt gen_tac >> strip_tac
+  >> ho_match_mp_tac pairs_rel_ind
+  >> rpt strip_tac
+  >> gvs[pair_rel_cases]
+  >> simp[Once pairs_rel_cases]
+  >> simp[pair_rel_cases]
+QED
+
+Theorem pairs_rel_loc:
+  ! refs' pairs refs l .
+    l < LENGTH pairs /\ pairs_rel refs' pairs refs 
+    ==>
+    pairs_loc 0 refs l < LENGTH refs /\
+    pair_rel refs' (EL l pairs) (EL (pairs_loc 0 refs l) refs)
+Proof
+  rpt strip_tac
+  >> dxrule_then assume_tac pairs_rel_FILTER
+  >> gvs[LIST_REL_EL_EQN, pairs_loc_FILTER]
+QED
+
+(*
 Inductive e_ce_rel:
 [~Val:]
-  ml_v_vals' v mlv ∧
+  ml_v_vals v mlv ∧
   nsLookup env.v (Short valv) = SOME (mlv) ∧
   nsLookup env.v (Short var) = SOME kv ∧
   valv ≠ var
@@ -426,26 +708,88 @@ Inductive e_ce_rel:
   e_ce_rel (Exception s) var env kv $
     Con (SOME $ Short "Ex") [Lit $ StrLit $ explode s]
 End
+*)
+
+Inductive cps_rel:
+[~Val:]
+  ml_v_vals refs v mlv ∧
+  nsLookup env.v (Short t) = SOME (mlv) ∧
+  nsLookup env.v (Short k) = SOME kv ∧
+  t ≠ k
+  ⇒
+  cps_rel refs (Val v) k env kv $ App Opapp [Var (Short k); Var (Short t)]
+[~Exp:]
+  ce = cps_transform e ∧
+  nsLookup env.v (Short k) = SOME kv ∧
+  scheme_env env ∧
+  env_rel refs senv env
+  ⇒
+  cps_rel refs (Exp senv e) var env kv $ App Opapp [ce; Var (Short k)]
+[~Exception:]
+  cps_rel refs (Exception s) var env kv $
+    Con (SOME $ Short "Ex") [Lit $ StrLit $ explode s]
+End
+
+Theorem env_rel_FEMPTY[simp]:
+  ∀ refs env . env_rel refs FEMPTY env
+Proof
+  simp[env_rel_cases, FEVERY_FEMPTY]
+QED
+
+Theorem env_rel_non_var[simp]:
+  ! refs se env envv var v .
+    (! x . var <> "var" ++ x)
+    ==>
+    env_rel refs se (env with v := nsBind var v envv) = env_rel refs se (env with v := envv)
+Proof
+  simp[env_rel_cases]
+QED
+
+Theorem scheme_env_sub:
+  ∀ env envv var v .
+    ¬ MEM var scheme_runtime_funs
+    ⇒
+   (scheme_env (env with v := nsBind var v envv) ⇔ scheme_env (env with v := envv))
+Proof
+  simp[scheme_runtime_funs_def, scheme_env_def]
+QED
+
+val scheme_env_tac = irule_at (Pat ‘scheme_env _’) $ iffRL scheme_env_sub >> simp[scheme_runtime_funs_def];
 
 Theorem compile_in_rel:
   ∀ p st env .
     scheme_env env
     ⇒
-    ∃ st' env' var mle k kv .
-      e_ce_rel (Exp p) var env' kv mle ∧
-      cont_rel k kv ∧
+    ∃ st' env' var mle ks kv .
+      cps_rel st.refs (Exp FEMPTY p) var env' kv mle ∧
+      cont_rel st.refs ks kv ∧
       evaluate st env [compile_scheme_prog p] = evaluate st' env' [mle]
 Proof
-  simp[Once e_ce_rel_cases, compile_scheme_prog_def]
+  simp[Once cps_rel_cases, compile_scheme_prog_def]
   >> rpt strip_tac
-  >> rpt (pairarg_tac >> gvs[])
   >> simp[Ntimes evaluate_def 2, nsOptBind_def]
   >> irule_at (Pos last) EQ_REFL
-  >> simp[]
   >> simp[Once cont_rel_cases]
-  >> gvs[scheme_env_def]
+  >> scheme_env_tac
   >> metis_tac[]
 QED
+
+Theorem scheme_cons_lookup:
+  ! env . scheme_env env ==> EVERY (\c . nsLookup env.c (Short c) = nsLookup scheme_cons_env (Short c)) scheme_conses
+Proof
+  rpt strip_tac
+  >> gvs[scheme_env_def, scheme_cons_env_def, scheme_conses_def, nsLookup_def]
+QED
+
+Theorem scheme_app_cons_lookup:
+  ! env . scheme_env_app env ==> EVERY (\c . nsLookup env.c (Short c) = nsLookup scheme_cons_env (Short c)) scheme_conses
+Proof
+  rpt strip_tac
+  >> gvs[scheme_env_app_def, scheme_cons_env_def, scheme_conses_def, nsLookup_def]
+QED
+
+val _ = augment_srw_ss $ single $ rewrites $ BODY_CONJUNCTS $ SRULE [IMP_CONJ_THM] $ RESTR_EVAL_RULE [``scheme_env``] scheme_cons_lookup;
+val _ = augment_srw_ss $ single $ rewrites $ BODY_CONJUNCTS $ SRULE [IMP_CONJ_THM] $ RESTR_EVAL_RULE [``scheme_env_app``] scheme_app_cons_lookup;
 
 (*
 open scheme_to_cakeProofTheory;
@@ -481,20 +825,22 @@ Theorem cps_app_ts_distinct:
     t ≠ "k" ∧
     ¬ MEM "t" ts ∧
     ¬ MEM "k" ts ∧
-    ¬ MEM t vconses ∧
-    EVERY (λ t. ¬ MEM t vconses) ts ∧
+    ¬ MEM t scheme_runtime_funs ∧
+    EVERY (λ t. ¬ MEM t scheme_runtime_funs) ts ∧
     (∀ x . t ≠ "var" ++ x) ∧
     EVERY (λ t. ∀ x . t ≠ "var" ++ x) ts
 Proof
   Induct_on ‘vs’
   >> simp[cps_app_ts_def]
   >> rpt (pairarg_tac >> gvs[])
+  >> gvs[scheme_runtime_funs_def]
   >> drule_then mp_tac $ GSYM cps_app_ts_res
   >> strip_tac
   >> qpat_x_assum ‘_ = t’ $ assume_tac o GSYM
   >> simp[]
   >> qpat_assum ‘∀ _ . _ ⇒ _’ $ irule_at (Pos hd) o SRULE []
-  >> irule_at (Pos last) str_not_num
+  >> simp[]
+  >> irule_at Any str_not_num
   >> simp[isDigit_def]
 QED
 
@@ -516,7 +862,7 @@ Proof
   >> gvs[scheme_env_def]
 QED
 
-Theorem map_reverse[simp]:
+Theorem map_reverse(*[simp]*):
   ∀ xs f . MAP f (REVERSE xs) = REVERSE (MAP f xs)
 Proof
   Induct >> simp[]
@@ -563,9 +909,21 @@ Proof
   simp[eval_eq_def]
 QED
 
+Definition val_eval_def:
+  val_eval st env k t = evaluate st env [App Opapp [Var (Short k); Var (Short t)]]
+End
+
+Definition exp_eval_def:
+  exp_eval st env e k = evaluate st env [App Opapp [cps_transform e; Var (Short k)]]
+End
+
+Definition ex_eval_def:
+  ex_eval st env s = evaluate st env [Con (SOME $ Short "Ex") [Lit $ StrLit s]]
+End
+
 Theorem preservation_of_sadd_body:
   ∀ vs mlvs .
-    LIST_REL ml_v_vals' vs mlvs
+    LIST_REL ml_v_vals vs mlvs
     ⇒
   ∀ store st env n k kv .
     cont_rel k kv ∧
@@ -612,10 +970,10 @@ Proof
     >> simp[GSYM eval_eq_def]
     >> irule_at (Pos hd) eval_eq_trivial
     >> last_assum $ irule_at (Pos hd)
-    >> simp[Once e_ce_rel_cases, sadd_def, Once ml_v_vals'_cases,
+    >> simp[Once e_ce_rel_cases, sadd_def, Once ml_v_vals_cases,
       env_rel_cases, FEVERY_FEMPTY]
   )
-  >> gvs[Once ml_v_vals'_cases]
+  >> gvs[Once ml_v_vals_cases]
   >> gvs[vcons_list_def]
   >~ [‘SNum m’] >- (
     simp[sadd_def]
@@ -647,7 +1005,7 @@ QED
 
 Theorem preservation_of_smul_body:
   ∀ vs mlvs .
-    LIST_REL ml_v_vals' vs mlvs
+    LIST_REL ml_v_vals vs mlvs
     ⇒
   ∀ store st env n k kv .
     cont_rel k kv ∧
@@ -694,10 +1052,10 @@ Proof
     >> simp[GSYM eval_eq_def]
     >> irule_at (Pos hd) eval_eq_trivial
     >> last_assum $ irule_at (Pos hd)
-    >> simp[Once e_ce_rel_cases, smul_def, Once ml_v_vals'_cases,
+    >> simp[Once e_ce_rel_cases, smul_def, Once ml_v_vals_cases,
       env_rel_cases, FEVERY_FEMPTY]
   )
-  >> gvs[Once ml_v_vals'_cases]
+  >> gvs[Once ml_v_vals_cases]
   >> gvs[vcons_list_def]
   >~ [‘SNum m’] >- (
     simp[smul_def]
@@ -729,7 +1087,7 @@ QED
 
 Theorem preservation_of_sminus_body:
   ∀ vs mlvs .
-    LIST_REL ml_v_vals' vs mlvs
+    LIST_REL ml_v_vals vs mlvs
     ⇒
   ∀ store (st:'ffi state) env n k kv .
     cont_rel k kv ∧
@@ -788,7 +1146,7 @@ Proof
   >> Cases_on ‘mlvs’
   >> simp[vcons_list_def]
   >> strip_tac
-  >> gvs[Once ml_v_vals'_cases]
+  >> gvs[Once ml_v_vals_cases]
   >~ [‘SNum i’] >- (
     simp[Ntimes evaluate_def 3]
     >> simp[can_pmatch_all_def, pmatch_def, nsLookup_def,
@@ -810,7 +1168,7 @@ Proof
         build_conv_def, nsOptBind_def, opn_lookup_def]
       >> simp[GSYM eval_eq_def]
       >> irule_at (Pos hd) eval_eq_trivial
-      >> simp[sminus_def, Once e_ce_rel_cases, Once ml_v_vals'_cases,
+      >> simp[sminus_def, Once e_ce_rel_cases, Once ml_v_vals_cases,
         env_rel_cases, FEVERY_FEMPTY]
     )
     >> qrefine ‘ck+3’
@@ -879,9 +1237,9 @@ Proof
       >> irule_at (Pos hd) eval_eq_trivial
       >> simp[env_rel_cases, FEVERY_FEMPTY]
       >> qpat_assum ‘cont_rel _ _’ $ irule_at (Pos hd)
-      >> simp[Once e_ce_rel_cases, Once ml_v_vals'_cases]
+      >> simp[Once e_ce_rel_cases, Once ml_v_vals_cases]
     )
-    >> gvs[Once ml_v_vals'_cases]
+    >> gvs[Once ml_v_vals_cases]
     >~ [‘SNum m’] >- (
       simp[sadd_def, vcons_list_def]
       >> simp[evaluate_def, do_opapp_def, do_app_def,
@@ -933,7 +1291,7 @@ QED
 Theorem preservation_of_proc:
 ∀ (st:'ffi state) inner n n' m m' env env' mlenv var kv n xs xp e e' ce k args vs mlvs store store' .
   valid_val store (Proc env xs xp e) ∧
-  LIST_REL ml_v_vals' vs mlvs ∧
+  LIST_REL ml_v_vals vs mlvs ∧
   EVERY (valid_val store) vs ∧
   valid_cont store k ∧
   cont_rel k kv ∧
@@ -1003,7 +1361,7 @@ Proof
     >> simp[]
     >> rpt (pairarg_tac >> gvs[])
     >> gvs[fresh_loc_def, store_entry_rel_cases]
-    >> simp[Once ml_v_vals'_cases]
+    >> simp[Once ml_v_vals_cases]
     >> simp[Once e_ce_rel_cases]
     >> irule_at Any EQ_REFL
     >> simp[]
@@ -1228,7 +1586,7 @@ Theorem preservation_of_letinit:
   ∀ (st:'ffi state) mlenv mlvs store env e k kv var xvs ts .
     EVERY (FDOM env) (MAP FST xvs) ∧
     EVERY (valid_val store) (MAP SND xvs) ∧
-    LIST_REL ml_v_vals' (MAP SND xvs) mlvs ∧
+    LIST_REL ml_v_vals (MAP SND xvs) mlvs ∧
     LIST_REL (λx mlv. nsLookup mlenv.v (Short x) = SOME mlv) ts mlvs ∧
     cont_rel k kv ∧ nsLookup mlenv.v (Short var) = SOME kv ∧
     scheme_env mlenv ∧
@@ -1290,161 +1648,350 @@ Proof
   >> simp[store_entry_rel_cases])
 QED
 
+Theorem state_ffi_trivial[simp]:
+  ! st:'ffi state . st with ffi := st.ffi = st
+Proof
+  simp[state_component_equality]
+QED
+
+Theorem state_refs_trivial[simp]:
+  ! st:'ffi state . st with refs := st.refs = st
+Proof
+  simp[state_component_equality]
+QED
+
+fun dup n x = if n = 0 then [] else x::dup (n-1) x;
+
+fun reduce_to_cps ck (thms:thm list) = EVERY (dup ck $ qrefine ‘ck+1’)
+    >> simp([GSYM exp_eval_def, GSYM val_eval_def, GSYM ex_eval_def, do_opapp_def, evaluate_def,
+            do_con_check_def, build_conv_def, dec_clock_def, nsOptBind_def,
+            do_app_def, can_pmatch_all_def, pmatch_def, store_lookup_def,
+            same_type_def, same_ctor_def, pat_bindings_def, store_assign_def, store_v_same_type_def]
+         @ thms)
+    >> simp([exp_eval_def, val_eval_def, ex_eval_def] @ thms);
+
+Theorem application_preservation:
+  ∀ sst sst' env env' fn vs e' ks ks' (st : 'ffi state) t mlfn ts mlvs mlenv k kv mle .
+    application sst ks fn vs = (sst',ks',e') ∧
+    cont_rel st.refs ks kv ∧
+    store_rel sst st.refs ∧
+    nsLookup mlenv.v (Short k) = SOME kv ∧
+    ml_v_vals st.refs fn mlfn ∧
+    nsLookup mlenv.v (Short t) = SOME mlfn ∧
+    LIST_REL (ml_v_vals st.refs) vs mlvs ∧
+    LIST_REL (λx mlv. nsLookup mlenv.v (Short x) = SOME mlv) ts mlvs ∧
+    scheme_env mlenv ∧
+    env_rel st.refs env mlenv
+    ⇒
+    ∃ ck st' mlenv' k' kv' mle' .
+      (∀ start . evaluate (st with clock := start + ck) mlenv
+        [App Opapp
+          [App Opapp
+            [App Opapp [Var (Short "app"); Var (Short k)];
+            Var (Short t)];
+          cons_list (MAP (Var o Short) ts)]]
+      =
+      evaluate (st' with clock := start) mlenv' [mle']) ∧
+      cont_rel st'.refs ks' kv' ∧
+      cps_rel st'.refs e' k' mlenv' kv' mle'∧
+      store_rel sst' st'.refs ∧
+      st.ffi = st'.ffi
+Proof
+  rpt strip_tac
+  >> drule_all_then assume_tac cons_list_val
+  >> drule $ cj 2 $ iffLR scheme_env_def
+  >> strip_tac
+  >> gvs[Once ml_v_vals_cases]
+  >> qrefine ‘ck+3’
+  >> simp[evaluate_def]
+  >> simp[do_opapp_def, dec_clock_def]
+  >> simp[Ntimes find_recfun_def 2, Ntimes build_rec_env_def 2]
+  >> simp[Ntimes evaluate_def 3]
+  >> simp[can_pmatch_all_def, pmatch_def, nsLookup_def,
+    same_type_def, same_ctor_def, evaluate_match_def,
+    pat_bindings_def]
+  >~ [`Prim SAdd`] >- (
+    drule $ cj 2 $ iffLR scheme_env_app_def
+    >> strip_tac
+    >> gvs[application_def]
+    >> qrefine ‘ck+2’
+    >> simp[evaluate_def]
+    >> simp[do_opapp_def, dec_clock_def]
+    >> simp[Ntimes find_recfun_def 2, Ntimes build_rec_env_def 2]
+    >> simp[Ntimes evaluate_def 2]
+    >> `? n . 0:int = n` by simp[]
+    >> pop_assum $ simp_tac std_ss o single
+    >> rpt $ pop_assum mp_tac
+    >> qid_spec_tac `n`
+    >> qid_spec_tac `vs`
+    >> qid_spec_tac `ts`
+    >> Induct_on `mlvs`
+    >> rpt strip_tac >- (
+      fs[cons_list_def, vcons_list_def, sadd_def]
+      >> rpt strip_tac
+      >> reduce_to_cps 0 [can_pmatch_all_def, pmatch_def, nsLookup_def,
+        same_type_def, same_ctor_def, evaluate_match_def,
+        pat_bindings_def]
+      >> simp[GSYM eval_eq_def]
+      >> irule_at (Pos hd) eval_eq_trivial
+      >> simp[Once cps_rel_cases, Once ml_v_vals_cases]
+    )
+    >> Cases_on `vs`
+    >> fs[]
+    >> Cases_on `ts`
+    >> fs[cons_list_def, vcons_list_def]
+    >> simp[Ntimes evaluate_def 2]
+    >> simp[can_pmatch_all_def, pmatch_def, nsLookup_def,
+      same_type_def, same_ctor_def, evaluate_match_def,
+      pat_bindings_def]
+    >> fs[Once ml_v_vals_cases]
+    >~ [`SNum i`]
+    >> simp[Ntimes evaluate_def 2]
+    >> simp[can_pmatch_all_def, pmatch_def, nsLookup_def,
+      same_type_def, same_ctor_def, evaluate_match_def,
+      pat_bindings_def]
+    >- (
+      qrefine ‘ck+3’
+      >> simp[evaluate_def]
+      >> simp[do_opapp_def, do_app_def, dec_clock_def, opn_lookup_def]
+      >> simp[Ntimes find_recfun_def 2, Ntimes build_rec_env_def 2]
+      >> simp[Ntimes evaluate_def 2]
+      >> simp[sadd_def]
+      >> simp[Once INT_ADD_COMM]
+      >> last_x_assum irule
+      >> simp[]
+      >> last_assum $ irule_at $ Pos last
+      >> irule cons_list_val
+      >> simp[]
+    )
+    >> simp[sadd_def]
+    >> simp[GSYM eval_eq_def]
+    >> irule_at (Pos hd) eval_eq_trivial
+    >> simp[Once cps_rel_cases]
+    >> first_assum $ irule_at $ Pos hd
+  )
+  >~ [`Prim SMul`] >- cheat
+  >~ [`Prim SMinus`] >- cheat
+  >~ [`Prim SEqv`] >- cheat
+  >~ [`Prim CallCC`] >- cheat
+  >~ [`Prim Cons`] >- cheat
+  >~ [`Prim Car`] >- cheat
+  >~ [`Prim Cdr`] >- cheat
+  >~ [`Proc se xs xp e`] >- (
+    pop_assum kall_tac
+    >> pop_assum kall_tac
+    >> rename1 `Closure proc_env _ _`
+    >> qrefine ‘ck+1’
+    >> simp[evaluate_def]
+    >> simp[do_opapp_def, dec_clock_def]
+    >> simp[Once evaluate_def]
+    >> gvs[application_def]
+    >> rpt (pairarg_tac >> gvs[])
+    >> qpat_x_assum `! _._` kall_tac
+    >> qpat_x_assum `scheme_env mlenv` kall_tac
+    >> qpat_x_assum `env_rel _ _ mlenv` kall_tac
+    >> qpat_x_assum `scheme_env_app _` kall_tac
+    >> rpt $ qpat_x_assum `nsLookup mlenv.v _ = _` kall_tac
+    >> qpat_x_assum `LIST_REL _ ts _` kall_tac
+    >> qpat_abbrev_tac `proc_env' = proc_env with v:= _`
+    >> `scheme_env proc_env'` by (unabbrev_all_tac >> rpt scheme_env_tac)
+    >> `env_rel st.refs se proc_env'` by simp[Abbr `proc_env'`]
+    >> `nsLookup proc_env'.v (Short "ts") = SOME (vcons_list mlvs)` by simp[Abbr `proc_env'`]
+    >> `nsLookup proc_env'.v (Short "k") = SOME kv` by simp[Abbr `proc_env'`]
+    >> qpat_x_assum `Abbrev _` kall_tac
+    >> qpat_x_assum `scheme_env proc_env` kall_tac
+    >> qpat_x_assum `env_rel _ _ proc_env` kall_tac
+    >> rpt $ pop_assum mp_tac
+    >> qid_spec_tac `se`
+    >> qid_spec_tac `proc_env'`
+    >> qid_spec_tac `sst`
+    >> qid_spec_tac `st`
+    >> qid_spec_tac `vs`
+    >> qid_spec_tac `mlvs`
+    >> Induct_on ‘xs’
+    >> rpt strip_tac
+    >> gvs[]
+    >- (
+      qpat_assum ‘cont_rel _ _ _’ $ irule_at (Pat ‘cont_rel _ _ _’)
+      >> Cases_on ‘xp’
+      >~ [`proc_ml _ (SOME _) _`] >- cheat
+      >> gvs[proc_ml_def]
+      >> Cases_on ‘vs’
+      >> gvs[parameterize_def]
+      >> reduce_to_cps 0 [can_pmatch_all_def, vcons_list_def, pmatch_def]
+      >> simp[GSYM eval_eq_def]
+      >> irule_at (Pos hd) eval_eq_trivial
+      >> simp[Once cps_rel_cases]
+    )
+    >> Cases_on ‘xp’
+    >~ [`proc_ml _ (SOME _) _`] >- cheat
+    >> simp[proc_ml_def]
+    >> Cases_on ‘vs’
+    >> gvs[parameterize_def] >- (
+      qpat_assum ‘cont_rel _ _ _’ $ irule_at (Pat ‘cont_rel _ _ _’)
+      >> reduce_to_cps 0 [can_pmatch_all_def, vcons_list_def, pmatch_def]
+      >> simp[GSYM eval_eq_def]
+      >> irule_at (Pos hd) eval_eq_trivial
+      >> simp[Once cps_rel_cases]
+    )
+    >> rpt (pairarg_tac >> gvs[])
+    >> reduce_to_cps 0 [can_pmatch_all_def, vcons_list_def, pmatch_def, store_alloc_def]
+val _ = (max_print_depth := 50);
+    >> qpat_abbrev_tac `new_st = st with refs := new_refs`
+    >> `st.ffi = new_st.ffi` by (unabbrev_all_tac >> simp[])
+    >> pop_assum $ simp o single
+    >> last_x_assum irule
+    >> unabbrev_all_tac
+    >> simp[]
+    >> irule_at Any EQ_REFL
+    >> rpt scheme_env_tac
+    >> first_assum $ irule_at $ Pat `parameterize _ _ _ _ _ _ = _`
+    >> gvs[fresh_loc_def]
+    >> simp[cont_rel_mono]
+    >> strip_tac >- (
+      irule LIST_REL_mono
+      >> last_assum $ irule_at $ Pos last
+      >> rpt strip_tac
+      >> simp[ml_v_vals_mono]
+    )
+    >> strip_tac >- (
+      irule env_rel_alloc
+      >> gvs[env_rel_cases]
+      >> rename1 `explode x`
+      >> Cases_on ‘x ∈ FDOM env’ >- (
+        simp[FEVERY_DEF]
+        >> strip_tac
+        >> rename1 `x' = x`
+        >> Cases_on ‘x' = x’
+        >> gvs[] >- (
+          drule $ cj 1 $ iffLR EVERY2_EVERY
+          >> simp[GSYM muts_loc_alloc_same]
+          >> simp[muts_loc_FILTER]
+        )
+        >> strip_tac
+        >> gvs[FEVERY_DEF]
+        >> simp[FAPPLY_FUPDATE_THM]
+      )
+      >> irule $ cj 2 FEVERY_STRENGTHEN_THM
+      >> simp[]
+      >> drule_then assume_tac $ cj 1 $ iffLR EVERY2_EVERY
+      >> simp[FEVERY_DEF]
+      >> rpt strip_tac
+      >> ‘x ≠ h’ by (strip_tac >> gvs[])
+      >> gvs[FEVERY_DEF]
+    )
+
+    >> qpat_assum ‘scheme_env mlenv’ $ simp
+      o curry ((::) o swap) [scheme_env_def]
+      o SRULE [scheme_env_def]
+    >> gvs[fresh_loc_def]
+    >> simp[SNOC_APPEND, store_entry_rel_cases]
+    >> irule_at (Pos hd) EVERY_MONOTONIC
+    >> qpat_assum ‘EVERY _ store’ $ irule_at (Pos $ el 2)
+    >> strip_tac >- (
+      rpt strip_tac
+      >> irule OPTION_ALL_MONO
+      >> pop_assum $ irule_at (Pos last)
+      >> rpt strip_tac
+      >> irule valid_val_larger_store
+      >> pop_assum $ irule_at (Pos last)
+      >> simp[]
+    )
+    >> irule_at (Pos hd) valid_val_larger_store
+    >> qpat_assum ‘valid_store _ h'’ $ irule_at (Pos $ el 2)
+    >> simp[]
+    >> irule_at (Pos hd) EVERY_MONOTONIC
+    >> qpat_assum ‘EVERY _ t’ $ irule_at (Pos $ el 2)
+    >> strip_tac >- (
+      rpt strip_tac
+      >> irule valid_val_larger_store
+      >> pop_assum $ irule_at (Pos last)
+      >> simp[]
+    )
+    >> irule_at (Pos $ el 3) valid_cont_larger_store
+    >> qpat_assum ‘valid_cont _ k'’ $ irule_at (Pos $ el 2)
+    >> simp[Once valid_val_cases]
+    >> conj_asm1_tac >- (
+      gvs[can_lookup_cases]
+      >> irule $ cj 2 FEVERY_STRENGTHEN_THM
+      >> irule_at (Pos last) FEVERY_MONO
+      >> qpat_assum ‘FEVERY _ env’ $ irule_at (Pos $ el 2)
+      >> simp[]
+      >> PairCases
+      >> simp[]
+    )
+    >> simp[]
+    >> gvs[env_rel_cases]
+    >> strip_tac >- (
+      Cases_on ‘h ∈ FDOM env’ >- (
+        simp[FEVERY_DEF]
+        >> strip_tac
+        >> Cases_on ‘x = h’
+        >> gvs[] >- (
+          drule $ cj 1 $ iffLR EVERY2_EVERY
+          >> simp[]
+        )
+        >> strip_tac
+        >> gvs[FEVERY_DEF]
+        >> simp[FAPPLY_FUPDATE_THM]
+      )
+      >> irule $ cj 2 FEVERY_STRENGTHEN_THM
+      >> simp[]
+      >> drule_then assume_tac $ cj 1 $ iffLR EVERY2_EVERY
+      >> simp[FEVERY_DEF]
+      >> rpt strip_tac
+      >> ‘x ≠ h’ by (strip_tac >> gvs[])
+      >> gvs[FEVERY_DEF]
+    )
+    >> Cases_on ‘xp’
+    >> simp[]
+    >> irule static_scope_mono
+    >> gvs[Once valid_val_cases]
+    >> qpat_assum ‘static_scope _ _’ $ irule_at (Pos last)
+    >> simp[Ntimes INSERT_SING_UNION 2]
+    >> simp[SUBSET_DEF]
+  )
+  >> reduce_to_cps 0 []
+  >> simp[GSYM eval_eq_def]
+  >> irule_at (Pos hd) eval_eq_trivial
+  >> simp[Once cps_rel_cases]
+  >> first_assum $ irule_at $ Pos hd
+QED
+
 Theorem step_preservation:
-  ∀ store store' env env' e e' k k' (st : 'ffi state) mlenv var kv mle .
-  step (store, k, env, e) = (store', k', env', e') ∧
-  valid_state store k env e ∧
-  cont_rel k kv ∧
-  e_ce_rel e var mlenv kv mle ∧
-  env_rel env mlenv ∧
-  LIST_REL store_entry_rel store st.refs
-  ⇒
-  ∃ ck st' mlenv' var' kv' mle' .
-    (∀ start . evaluate (st with clock := start + ck) mlenv [mle]
-    =
-    evaluate (st' with clock := start) mlenv' [mle']) ∧
-    cont_rel k' kv' ∧
-    e_ce_rel e' var' mlenv' kv' mle' ∧
-    env_rel env' mlenv' ∧
-    LIST_REL store_entry_rel store' st'.refs ∧
-    (¬ terminating_state (store', k', env', e') ⇒ 0 < ck) ∧
-    st.ffi = st'.ffi
+  ∀ sst sst' env env' e e' ks ks' (st : 'ffi state) mlenv k kv mle .
+    step (sst, ks, e) = (sst', ks', e') ∧
+    valid_state sst ks e ∧
+    cont_rel st.refs ks kv ∧
+    cps_rel st.refs e k mlenv kv mle ∧
+    store_rel sst st.refs
+    ⇒
+    ∃ ck st' mlenv' k' kv' mle' .
+      (∀ start . evaluate (st with clock := start + ck) mlenv [mle]
+      =
+      evaluate (st' with clock := start) mlenv' [mle']) ∧
+      cont_rel st.refs ks' kv' ∧
+      cps_rel st.refs e' k' mlenv' kv' mle' ∧
+      store_rel sst' st'.refs ∧
+      (¬ terminating_state (sst', ks', e') ⇒ 0 < ck) ∧
+      st.ffi = st'.ffi
 Proof
   Cases_on ‘e’
   >> simp[terminating_state_def]
   >~ [‘Exception s’] >- (
-    simp[step_def, Once e_ce_rel_cases]
+    simp[step_def, Once cps_rel_cases]
     >> rpt strip_tac
     >> simp[GSYM eval_eq_def]
     >> irule_at (Pos hd) eval_eq_trivial
-    >> simp[Once e_ce_rel_cases, Once cont_rel_cases]
-    >> qexists ‘scheme_env7’
-    >> simp[scheme_env_def]
+    >> simp[Once cps_rel_cases, Once cont_rel_cases]
+    >> irule_at (Pos hd) basis_scheme_env
   )
-  >~ [‘Exp e’] >- (
+  >~ [‘Exp env e’] >- (
     Cases_on ‘e’
-    >> simp[step_def, Once e_ce_rel_cases]
-    >~ [‘Lit l’] >- (
-      simp[cps_transform_def]
-      >> rpt strip_tac
-      >> Cases_on ‘l’
-      >> simp[lit_to_val_def, to_ml_vals_def]
-      >> TRY CASE_TAC (*for Prim cases*)
-      >> TRY (Cases_on ‘b’) (*for Bool cases*)
-      >> gvs[lit_to_val_def, to_ml_vals_def]
-      >> qrefine ‘ck+1’
-      >> simp[SimpLHS, Ntimes evaluate_def 7, do_opapp_def,
-        do_con_check_def, build_conv_def, nsOptBind_def, dec_clock_def]
-      >> qpat_assum ‘scheme_env mlenv’ $ simp o single
-        o SRULE [scheme_env_def]
-      >> simp[GSYM eval_eq_def]
-      >> irule_at (Pos hd) eval_eq_trivial
-      >> simp[Once e_ce_rel_cases, Once ml_v_vals'_cases]
-      >> gvs[env_rel_cases]
-    )
-    >~ [‘Cond c te fe’] >- (
-      simp[cps_transform_def]
-      >> rpt strip_tac
-      >> qrefine ‘ck+1’
-      >> simp[SimpLHS, Ntimes evaluate_def 6, do_opapp_def,
-        nsOptBind_def, dec_clock_def]
-      >> simp[GSYM eval_eq_def]
-      >> irule_at (Pos hd) eval_eq_trivial
-      >> simp[Once e_ce_rel_cases, Once cont_rel_cases]
-      >> gvs[scheme_env_def, env_rel_cases]
-    )
-    >~ [‘Apply fn es’] >- (
-      simp[cps_transform_def]
-      >> rpt strip_tac
-      >> qrefine ‘ck+1’
-      >> simp[SimpLHS, Ntimes evaluate_def 6, do_opapp_def,
-        nsOptBind_def, dec_clock_def]
-      >> simp[GSYM eval_eq_def]
-      >> irule_at (Pos hd) eval_eq_trivial
-      >> simp[Once e_ce_rel_cases, Once cont_rel_cases]
-      >> gvs[scheme_env_def, env_rel_cases]
-    )
-    >~ [‘Begin es e’] >- (
-      Cases_on ‘es’
-      >> rpt strip_tac
-      >> gvs[cps_transform_def] >- (
-        qrefine ‘ck+1’
-        >> simp[SimpLHS, Ntimes evaluate_def 4, do_opapp_def,
-          nsOptBind_def, dec_clock_def]
-        >> simp[GSYM eval_eq_def]
-        >> irule_at (Pos hd) eval_eq_trivial
-        >> qpat_assum ‘cont_rel _ _’ $ irule_at (Pos hd)
-        >> simp[Once e_ce_rel_cases]
-        >> gvs[scheme_env_def, env_rel_cases]
-      )
-      >> qrefine ‘ck+1’
-      >> simp[SimpLHS, Ntimes evaluate_def 6, do_opapp_def,
-        nsOptBind_def, dec_clock_def]
-      >> simp[GSYM eval_eq_def]
-      >> irule_at (Pos hd) eval_eq_trivial
-      >> simp[Once e_ce_rel_cases, Once cont_rel_cases]
-      >> gvs[scheme_env_def, env_rel_cases]
-    )
-    >~ [‘Lambda xs xp e’] >- (
-      simp[cps_transform_def]
-      >> rpt strip_tac
-      >> qrefine ‘ck+1’
-      >> simp[Ntimes evaluate_def 7, do_opapp_def,
-        nsOptBind_def, dec_clock_def, do_con_check_def,
-        build_conv_def]
-      >> qpat_assum ‘scheme_env mlenv’ $ simp o single
-        o SRULE [scheme_env_def]
-      >> simp[GSYM eval_eq_def]
-      >> irule_at (Pos hd) eval_eq_trivial
-      >> last_assum $ irule_at (Pos hd)
-      >> simp[Once e_ce_rel_cases, Once ml_v_vals'_cases]
-      >> gvs[scheme_env_def, env_rel_cases]
-    )
-    >~ [‘Ident x’] >- (
-      simp[cps_transform_def]
-      >> rpt strip_tac
-      >> gvs[Once valid_state_cases]
-      >> gvs[Once static_scope_def]
-      >> gvs[Once $ GSYM SPECIFICATION]
-      >> qpat_assum ‘env_rel _ _’ $ drule_then assume_tac
-        o SRULE [env_rel_cases, FEVERY_DEF]
-      >> qpat_assum ‘can_lookup _ _’ $ drule_then assume_tac
-        o SRULE [can_lookup_cases, FEVERY_DEF]
-      >> qpat_assum ‘LIST_REL _ _ _’ $ mp_tac
-        o SRULE [LIST_REL_EL_EQN, store_entry_rel_cases]
-      >> strip_tac
-      >> pop_assum $ drule_then assume_tac
-      >> qrefine ‘ck+1’
-      >> simp[SimpLHS, Ntimes evaluate_def 7, do_opapp_def,
-        nsOptBind_def, dec_clock_def]
-      >> simp[can_pmatch_all_def, pmatch_def, evaluate_match_def,
-        do_app_def, store_lookup_def]
-      >> Cases_on ‘EL (env ' x) store’
-      >> gvs[]
-      >> simp[can_pmatch_all_def, pmatch_def, evaluate_match_def,
-        do_app_def, store_lookup_def]
-      >> qpat_assum ‘scheme_env mlenv’ $ simp o single
-        o SRULE [scheme_env_def]
-      >> simp[same_type_def, same_ctor_def, pat_bindings_def]
-      >> simp[GSYM eval_eq_def]
-      >> irule_at (Pos hd) eval_eq_trivial
-      >> simp[]
-      >> qpat_assum ‘cont_rel _ _’ $ irule_at (Pos hd)
-      >> simp[Once e_ce_rel_cases]
-      >> gvs[env_rel_cases]
-    )
-    >~ [‘Set x e’] >- (
-      simp[cps_transform_def]
-      >> rpt strip_tac
-      >> qrefine ‘ck+1’
-      >> simp[SimpLHS, Ntimes evaluate_def 6, do_opapp_def,
-        nsOptBind_def, dec_clock_def]
-      >> simp[GSYM eval_eq_def]
-      >> irule_at (Pos hd) eval_eq_trivial
-      >> simp[Once e_ce_rel_cases, Once cont_rel_cases]
-      >> gvs[scheme_env_def, env_rel_cases]
-    )
+    >> simp[step_def, Once cps_rel_cases]
     >~ [‘Letrec bs e’] >- (
+      cheat
+      (*
       Cases_on ‘bs’
       >> rpt strip_tac
       >> gvs[cps_transform_def] >- (
@@ -1493,8 +2040,11 @@ Proof
       >> simp[cps_app_ts_def]
       >> simp[Once e_ce_rel_cases]
       >> gvs[scheme_env_def, env_rel_cases]
+      *)
     )
     >~ [‘Letrecstar bs e’] >- (
+      cheat
+      (*
       simp[Once cps_transform_def]
       >> rpt strip_tac
       >> rpt (pairarg_tac >> gvs[])
@@ -1520,93 +2070,113 @@ Proof
       >> first_assum $ irule_at (Pos hd)
       >> qpat_assum ‘cont_rel _ _’ $ irule_at (Pos hd)
       >> simp[Once e_ce_rel_cases]
+      *)
     )
+    >~ [‘Begin es e’] >>> HEADGOAL $ Cases_on ‘es’
+    >> simp[cps_transform_def]
+    >~ [‘Lit l’] >>> HEADGOAL (
+      Cases_on ‘l’
+      >~ [`LitBool b`] >>> HEADGOAL $ Cases_on ‘b’ (*for Bool cases*)
+      >~ [`LitPrim p`] >>> HEADGOAL $ Cases_on `p`
+      >> simp[lit_to_val_def, lit_to_ml_val_def]
+    )
+    >> rpt strip_tac
+    >~ [‘Ident x’] >>> HEADGOAL (
+      gvs[Once valid_state_cases]
+      >> gvs[Once static_scope_def]
+      >> gvs[Once $ GSYM SPECIFICATION]
+      >> qpat_assum ‘env_rel _ _ _’ $ drule_then assume_tac
+        o SRULE [env_rel_cases, FEVERY_DEF]
+      >> qpat_assum ‘can_lookup _ _’ $ drule_then assume_tac
+        o SRULE [can_lookup_cases, FEVERY_DEF]
+      >> drule_all muts_rel_loc >> strip_tac
+      >> gvs[store_entry_rel_cases]
+    )
+    >> reduce_to_cps 1 []
+    >> simp[GSYM eval_eq_def]
+    >> irule_at (Pos hd) eval_eq_trivial
+    >> TRY $ qpat_assum ‘cont_rel _ _ _’ $ irule_at (Pos hd)
+    >> simp[Once cps_rel_cases]
+    >> simp[Once ml_v_vals_cases, Once cont_rel_cases]
+    >> rpt scheme_env_tac
   )
   >~ [‘Val v’] >- (
-    Cases_on ‘k’
+    Cases_on ‘ks’
     >- (
       simp[step_def, return_def]
       >> rw[]
       >> simp[GSYM eval_eq_def]
       >> irule_at (Pos hd) eval_eq_trivial
-      >> simp[env_rel_cases, FEVERY_FEMPTY]
-      >> metis_tac[]
+      >> simp[]
+      >> rpt $ first_assum $ irule_at Any
     )
     >> PairCases_on ‘h’
     >> Cases_on ‘∃ te fe . h1 = CondK te fe’ >- (
       gvs[]
       >> simp[step_def, return_def]
-      >> simp[Once e_ce_rel_cases, Once cont_rel_cases]
-      >> simp[Once ml_v_vals'_cases]
+      >> simp[Once cps_rel_cases, Once cont_rel_cases]
+      >> simp[Once ml_v_vals_cases]
       >> rpt strip_tac
       >> gvs[]
-      >> qrefine ‘ck+1’
-      >> simp[SimpLHS, Ntimes evaluate_def 6, do_con_check_def,
-        build_conv_def, scheme_env_def, do_opapp_def,
-      can_pmatch_all_def, pmatch_def, dec_clock_def]
-      >> qpat_assum ‘scheme_env env''’ $ simp o curry ((::) o swap) [
-          same_type_def, same_ctor_def, do_opapp_def,
-          evaluate_match_def, pmatch_def, pat_bindings_def]
-        o SRULE [scheme_env_def]
+      >> simp[Once evaluate_def]
+      >> reduce_to_cps 1 []
       >> simp[GSYM eval_eq_def]
       >> irule_at (Pos hd) eval_eq_trivial
-      >> gvs[]
-      >> qpat_assum ‘cont_rel _ _’ $ irule_at (Pos hd)
-      >> simp[Once e_ce_rel_cases]
-      >> gvs[scheme_env_def, env_rel_cases]
+      >> qpat_assum ‘cont_rel _ _ _’ $ irule_at (Pos hd)
+      >> simp[Once cps_rel_cases]
+      >> scheme_env_tac
     )
     >> Cases_on ‘∃ es e . h1 = BeginK es e’ >- (
       gvs[]
       >> Cases_on ‘es’
       >> rpt strip_tac
-      >> gvs[Once cont_rel_cases, Once e_ce_rel_cases]
+      >> gvs[Once cont_rel_cases, Once cps_rel_cases]
       >> gvs[cps_transform_def, step_def, return_def]
-      >> qrefine ‘ck+1’
-      >> simp[SimpLHS, Ntimes evaluate_def 4, do_opapp_def,
-        nsOptBind_def, dec_clock_def] >- (
-        simp[GSYM eval_eq_def]
-        >> irule_at (Pos hd) eval_eq_trivial
-        >> qpat_assum ‘cont_rel _ _’ $ irule_at (Pos hd)
-        >> simp[Once e_ce_rel_cases]
-        >> gvs[scheme_env_def, env_rel_cases]
-      )
-      >> simp[SimpLHS, Ntimes evaluate_def 2, nsOptBind_def]
+      >> simp[Once evaluate_def]
+      >> reduce_to_cps 1 []
       >> simp[GSYM eval_eq_def]
       >> irule_at (Pos hd) eval_eq_trivial
-      >> simp[Once e_ce_rel_cases, Once cont_rel_cases]
-      >> gvs[scheme_env_def, env_rel_cases]
+      >> simp[Once cps_rel_cases]
+      >> simp[Once cont_rel_cases]
+      >> rpt scheme_env_tac
     )
     >> Cases_on ‘∃ x . h1 = SetK x’ >- (
       gvs[]
-      >> simp[step_def, return_def, Once e_ce_rel_cases, refunc_set_def,
+      >> simp[step_def, return_def, Once cps_rel_cases, refunc_set_def,
         Once cont_rel_cases, cps_transform_def, cps_app_ts_def]
       >> rpt strip_tac
-      >> simp[]
-      >> gvs[Once valid_state_cases]
-      >> qpat_x_assum ‘valid_cont _ _’ $ mp_tac
-        o SRULE [Once valid_val_cases]
-      >> strip_tac
-      >> qpat_assum ‘env_rel h0 _’ $ drule_then assume_tac
+      >> gvs[Once valid_state_cases, Once valid_cont_cases]
+      >> qpat_assum ‘env_rel _ _ _’ $ drule_then assume_tac
         o SRULE [env_rel_cases, FEVERY_DEF, SPECIFICATION]
-      >> qpat_assum ‘can_lookup h0 _’ $ drule_then assume_tac
+      >> qpat_assum ‘can_lookup _ _’ $ drule_then assume_tac
         o SRULE [can_lookup_cases, FEVERY_DEF, SPECIFICATION]
-      >> drule_then assume_tac EVERY2_LENGTH
-      >> drule_all_then assume_tac $ cj 2 $ iffLR LIST_REL_EL_EQN
+      >> drule_all muts_rel_loc >> strip_tac
       >> gvs[store_entry_rel_cases]
-      >> qrefine ‘ck+1’
-      >> simp[Ntimes evaluate_def 13, do_con_check_def, nsOptBind_def,
-        build_conv_def, scheme_env_def, do_opapp_def, dec_clock_def,
-        do_app_def, store_assign_def, store_v_same_type_def]
-      >> qpat_assum ‘scheme_env _’ $ simp o single
-        o SRULE [scheme_env_def]
+      >> simp[Once evaluate_def]
+      >> reduce_to_cps 1 []
       >> simp[GSYM eval_eq_def]
       >> irule_at (Pos hd) eval_eq_trivial
       >> simp[]
-      >> qpat_assum ‘cont_rel _ _’ $ irule_at (Pos hd)
-      >> simp[Once e_ce_rel_cases, Once ml_v_vals'_cases]
-      >> gvs[env_rel_cases]
-      >> irule EVERY2_LUPDATE_same
+      >> qpat_assum ‘cont_rel _ _ _’ $ irule_at (Pos hd)
+      >> simp[Once cps_rel_cases, Once ml_v_vals_cases]
+      >> (strip_tac >- (
+        irule muts_rel_LUPDATE_same
+        >> irule_at (Pos hd) muts_rel_mono
+        >> qpat_assum `muts_rel _ _ _` $ irule_at Any
+        >> rpt strip_tac
+        >> gvs[store_entry_rel_cases, ml_v_vals_LUPDATE_same]
+      )
+      >> irule pairs_rel_LUPDATE_diff
+      >> irule_at (Pos hd) pairs_rel_mono
+      >> qpat_assum `pairs_rel _ _ _` $ irule_at Any
+      >> rpt strip_tac
       >> simp[store_entry_rel_cases]
+      >> irule_at Any EQ_REFL
+      >> irule_at Any ml_v_vals_LUPDATE_same
+      >> rpt $ first_assum $ irule_at $ Pos hd
+      >> rpt strip_tac
+      >> gvs[Once pair_rel_cases]
+      >> simp[Once pair_rel_cases, ml_v_vals_LUPDATE_same])
     )
     >> Cases_on ‘∃ xvs x bs e . h1 = LetinitK xvs x bs e’ >- (
       gvs[]
@@ -1666,11 +2236,11 @@ Proof
       >> rpt (pairarg_tac >> gvs[])
       >> qpat_assum ‘LIST_REL _ ts mlvs’ $ assume_tac
       >> dxrule_then assume_tac EVERY2_LENGTH
-      >> qpat_assum ‘LIST_REL ml_v_vals' _ mlvs’ $ assume_tac
+      >> qpat_assum ‘LIST_REL ml_v_vals _ mlvs’ $ assume_tac
       >> dxrule_then assume_tac EVERY2_LENGTH
       >> gvs[]
       >> qpat_assum ‘cont_rel _ _’ $ irule_at (Pos hd)
-      >> qpat_assum ‘LIST_REL ml_v_vals' _ _’ $ irule_at (Pos $ el 2)
+      >> qpat_assum ‘LIST_REL ml_v_vals _ _’ $ irule_at (Pos $ el 2)
       >> drule $ GSYM cps_app_ts_distinct
       >> strip_tac
       >> simp[]
@@ -1689,36 +2259,34 @@ Proof
     )
     >> Cases_on ‘∃ e es . h1 = ApplyK NONE (e::es)’ >- (
       gvs[]
-      >> simp[step_def, return_def, Once e_ce_rel_cases,
+      >> simp[step_def, return_def, Once cps_rel_cases,
         Once cont_rel_cases, cps_transform_def, cps_app_ts_def]
       >> rpt strip_tac
-      >> qrefine ‘ck+1’
-      >> simp[Ntimes evaluate_def 6, do_opapp_def,
-        nsOptBind_def, dec_clock_def]
+      >> simp[evaluate_def]
+      >> reduce_to_cps 1 []
       >> simp[GSYM eval_eq_def]
       >> irule_at (Pos hd) eval_eq_trivial
-      >> simp[Once e_ce_rel_cases, Once cont_rel_cases]
+      >> simp[Once cps_rel_cases, Once cont_rel_cases]
       >> simp[cps_app_ts_def]
-      >> gvs[scheme_env_def, env_rel_cases]
+      >> rpt scheme_env_tac
     )
     >> Cases_on ‘∃ fn vs e es . h1 = ApplyK (SOME (fn, vs)) (e::es)’ >- (
       gvs[]
-      >> simp[step_def, return_def, Once e_ce_rel_cases,
+      >> simp[step_def, return_def, Once cps_rel_cases,
         Once cont_rel_cases, cps_transform_def, cps_app_ts_def]
       >> rpt strip_tac
-      >> qrefine ‘ck+1’
-      >> simp[Ntimes evaluate_def 6, do_opapp_def,
-        nsOptBind_def, dec_clock_def]
+      >> simp[evaluate_def]
+      >> reduce_to_cps 1 []
       >> simp[GSYM eval_eq_def]
       >> irule_at (Pos hd) eval_eq_trivial
-      >> simp[Once e_ce_rel_cases, Once cont_rel_cases]
+      >> simp[Once cps_rel_cases, Once cont_rel_cases]
       >> simp[PULL_EXISTS]
       >> irule_at (Pos hd) EQ_REFL
-      >> qpat_assum ‘cont_rel _ _’ $ irule_at (Pos hd)
+      >> qpat_assum ‘cont_rel _ _ _’ $ irule_at (Pos hd)
       >> simp[cps_app_ts_def]
       >> rpt (pairarg_tac >> gvs[])
-      >> qpat_assum ‘ml_v_vals' _ _’ $ irule_at Any
-      >> qpat_assum ‘LIST_REL ml_v_vals' _ _’ $ irule_at Any
+      >> qpat_assum ‘ml_v_vals _ _ _’ $ irule_at Any
+      >> qpat_assum ‘LIST_REL (ml_v_vals _) _ _’ $ irule_at Any
       >> drule $ GSYM cps_app_ts_distinct
       >> strip_tac
       >> simp[]
@@ -1735,13 +2303,18 @@ Proof
         >> strip_tac
         >> gvs[]
       )
-      >> gvs[scheme_env_def, env_rel_cases]
+      >> rpt scheme_env_tac
     )
     >> Cases_on ‘h1 = ApplyK NONE []’ >- (
       gvs[]
-      >> simp[step_def, return_def, Once e_ce_rel_cases, Once cont_rel_cases]
-      >> simp[Once ml_v_vals'_cases]
+      >> simp[step_def, return_def, Once cps_rel_cases, Once cont_rel_cases]
+      >> simp[Once ml_v_vals_cases]
       >> rpt strip_tac
+      >> gvs[]
+      >> simp[Once evaluate_def]
+      >> reduce_to_cps 1 []
+      >> cheat
+
       >> gvs[application_def, sadd_def, smul_def, sminus_def,
         seqv_def, cps_transform_def, cons_list_def]
       >> qrefine ‘ck+2’
@@ -1760,7 +2333,7 @@ Proof
         >> simp[Once evaluate_def]
         >> simp[GSYM eval_eq_def]
         >> irule_at (Pos hd) eval_eq_trivial
-        >> simp[Once e_ce_rel_cases]
+        >> simp[Once cps_rel_cases]
         >> last_assum $ irule_at (Pos hd)
         >> simp[env_rel_cases, FEVERY_FEMPTY]
       )
@@ -1771,7 +2344,7 @@ Proof
         >> simp[Once evaluate_def]
         >> simp[GSYM eval_eq_def]
         >> irule_at (Pos hd) eval_eq_trivial
-        >> simp[Once e_ce_rel_cases]
+        >> simp[Once cps_rel_cases]
         >> last_assum $ irule_at (Pos hd)
         >> simp[env_rel_cases, FEVERY_FEMPTY]
       )
@@ -1782,7 +2355,7 @@ Proof
         >> simp[Once evaluate_def]
         >> simp[GSYM eval_eq_def]
         >> irule_at (Pos hd) eval_eq_trivial
-        >> simp[Once e_ce_rel_cases]
+        >> simp[Once cps_rel_cases]
         >> last_assum $ irule_at (Pos hd)
         >> simp[env_rel_cases, FEVERY_FEMPTY]
       )
@@ -1791,7 +2364,7 @@ Proof
         >> simp[Once evaluate_def]
         >> simp[GSYM eval_eq_def]
         >> irule_at (Pos hd) eval_eq_trivial
-        >> simp[Once e_ce_rel_cases]
+        >> simp[Once cps_rel_cases]
         >> last_assum $ irule_at (Pos hd)
         >> simp[env_rel_cases, FEVERY_FEMPTY]
       )
@@ -1800,7 +2373,7 @@ Proof
         >> simp[Once evaluate_def]
         >> simp[GSYM eval_eq_def]
         >> irule_at (Pos hd) eval_eq_trivial
-        >> simp[Once e_ce_rel_cases]
+        >> simp[Once cps_rel_cases]
         >> last_assum $ irule_at (Pos hd)
         >> simp[env_rel_cases, FEVERY_FEMPTY]
       )
@@ -1819,7 +2392,7 @@ Proof
         >> simp[GSYM eval_eq_def]
         >> irule_at (Pos hd) eval_eq_trivial
         >> last_assum $ irule_at (Pos hd)
-        >> simp[Once e_ce_rel_cases, Once ml_v_vals'_cases]
+        >> simp[Once cps_rel_cases, Once ml_v_vals_cases]
         >> simp[env_rel_cases, FEVERY_FEMPTY]
       )
       >~ [‘"SMul"’] >- (
@@ -1829,7 +2402,7 @@ Proof
         >> simp[GSYM eval_eq_def]
         >> irule_at (Pos hd) eval_eq_trivial
         >> last_assum $ irule_at (Pos hd)
-        >> simp[Once e_ce_rel_cases, Once ml_v_vals'_cases]
+        >> simp[Once cps_rel_cases, Once ml_v_vals_cases]
         >> simp[env_rel_cases, FEVERY_FEMPTY]
       )
       >~ [‘Proc _ _ _ _’] >- (
@@ -1853,11 +2426,20 @@ Proof
       )
       >> simp[GSYM eval_eq_def]
       >> irule_at (Pos hd) eval_eq_trivial
-      >> simp[Once e_ce_rel_cases]
+      >> simp[Once cps_rel_cases]
       >> simp[env_rel_cases, FEVERY_FEMPTY]
       >> last_assum $ irule_at Any
     )
     >> Cases_on ‘∃ fn vs . h1 = ApplyK (SOME (fn, vs)) []’ >- (
+      gvs[]
+      >> simp[step_def, return_def, Once cps_rel_cases]
+      >> rpt strip_tac
+      >> gvs[Once cont_rel_cases, Excl "MAP"]
+      >> simp[Once evaluate_def]
+      >> reduce_to_cps 1 [Excl "MAP"]
+      >> gvs[cps_transform_def, Excl "MAP"]
+      >> simp_tac std_ss [Once $ GSYM MAP_REVERSE]
+
       gvs[]
       >> simp[step_def, return_def, Once e_ce_rel_cases,
         Once cont_rel_cases]
@@ -1873,7 +2455,7 @@ Proof
       env''.v).v (Short x) = SOME v') (REVERSE (t'::ts)) (REVERSE (mlv::mlvs))’ >- (
         strip_tac
         >> drule_all_then assume_tac cons_list_val
-        >> gvs[Once ml_v_vals'_cases]
+        >> gvs[Once ml_v_vals_cases]
         >> gvs[application_def]
         >> qpat_assum ‘scheme_env env''’ $ simp o single o SRULE [scheme_env_def]
         >> simp[Ntimes find_recfun_def 2, Ntimes build_rec_env_def 2]
@@ -1998,13 +2580,13 @@ Proof
               same_type_def, same_ctor_def, evaluate_match_def,
               pat_bindings_def]
             >> Cases_on ‘∃ n . x = SNum n’ >- (
-              gvs[Once ml_v_vals'_cases]
+              gvs[Once ml_v_vals_cases]
               >> simp[Ntimes evaluate_def 8]
               >> simp[can_pmatch_all_def, pmatch_def, nsLookup_def,
                 same_type_def, same_ctor_def, evaluate_match_def,
                 pat_bindings_def, do_con_check_def, build_conv_def]
               >> Cases_on ‘∃ m . v = SNum m’ >- (
-                gvs[Once ml_v_vals'_cases]
+                gvs[Once ml_v_vals_cases]
                 >> simp[Ntimes evaluate_def 11, nsOptBind_def, do_app_def]
                 >> simp[can_pmatch_all_def, pmatch_def, nsLookup_def,
                   same_type_def, same_ctor_def, evaluate_match_def,
@@ -2015,11 +2597,11 @@ Proof
                 >> simp[env_rel_cases, FEVERY_FEMPTY]
                 >> qpat_assum ‘cont_rel _ _’ $ irule_at (Pos hd)
                 >> Cases_on ‘i=i'’
-                >> simp[Once e_ce_rel_cases, Once ml_v_vals'_cases,
+                >> simp[Once e_ce_rel_cases, Once ml_v_vals_cases,
                   Boolv_def, bool_type_num_def]
               )
               >> Cases_on ‘v’
-              >> gvs[Once ml_v_vals'_cases]
+              >> gvs[Once ml_v_vals_cases]
               >> simp[Ntimes evaluate_def 8, nsOptBind_def]
               >> simp[can_pmatch_all_def, pmatch_def, nsLookup_def,
                 same_type_def, same_ctor_def, evaluate_match_def,
@@ -2028,17 +2610,17 @@ Proof
               >> irule_at (Pos hd) eval_eq_trivial
               >> simp[env_rel_cases, FEVERY_FEMPTY]
               >> qpat_assum ‘cont_rel _ _’ $ irule_at (Pos hd)
-              >> simp[Once e_ce_rel_cases, Once ml_v_vals'_cases,
+              >> simp[Once e_ce_rel_cases, Once ml_v_vals_cases,
                 Boolv_def, bool_type_num_def]
             )
             >> Cases_on ‘∃ b . x = SBool b’ >- (
-              gvs[Once ml_v_vals'_cases]
+              gvs[Once ml_v_vals_cases]
               >> simp[Ntimes evaluate_def 8]
               >> simp[can_pmatch_all_def, pmatch_def, nsLookup_def,
                 same_type_def, same_ctor_def, evaluate_match_def,
                 pat_bindings_def, do_con_check_def, build_conv_def]
               >> (Cases_on ‘∃ b' . v = SBool b'’ >- (
-                gvs[Once ml_v_vals'_cases]
+                gvs[Once ml_v_vals_cases]
                 >> simp[Ntimes evaluate_def 11, nsOptBind_def, do_app_def]
                 >> simp[can_pmatch_all_def, pmatch_def, nsLookup_def,
                   same_type_def, same_ctor_def, evaluate_match_def,
@@ -2048,11 +2630,11 @@ Proof
                 >> irule_at (Pos hd) eval_eq_trivial
                 >> simp[env_rel_cases, FEVERY_FEMPTY]
                 >> qpat_assum ‘cont_rel _ _’ $ irule_at (Pos hd)
-                >> simp[Once e_ce_rel_cases, Once ml_v_vals'_cases,
+                >> simp[Once e_ce_rel_cases, Once ml_v_vals_cases,
                   Boolv_def, bool_type_num_def]
               ))
               >> Cases_on ‘v’ >> gvs[]
-              >> gvs[Once ml_v_vals'_cases]
+              >> gvs[Once ml_v_vals_cases]
               >> simp[Ntimes evaluate_def 8, nsOptBind_def]
               >> simp[can_pmatch_all_def, pmatch_def, nsLookup_def,
                 same_type_def, same_ctor_def, evaluate_match_def,
@@ -2061,11 +2643,11 @@ Proof
               >> irule_at (Pos hd) eval_eq_trivial
               >> simp[env_rel_cases, FEVERY_FEMPTY]
               >> qpat_assum ‘cont_rel _ _’ $ irule_at (Pos hd)
-              >> simp[Once e_ce_rel_cases, Once ml_v_vals'_cases,
+              >> simp[Once e_ce_rel_cases, Once ml_v_vals_cases,
                 Boolv_def, bool_type_num_def]
             )
             >> Cases_on ‘x’ >> gvs[]
-            >> gvs[Once ml_v_vals'_cases]
+            >> gvs[Once ml_v_vals_cases]
             >> simp[Ntimes evaluate_def 9, nsOptBind_def]
             >> simp[can_pmatch_all_def, pmatch_def, nsLookup_def,
               same_type_def, same_ctor_def, evaluate_match_def,
@@ -2074,7 +2656,7 @@ Proof
             >> irule_at (Pos hd) eval_eq_trivial
             >> simp[env_rel_cases, FEVERY_FEMPTY]
             >> qpat_assum ‘cont_rel _ _’ $ irule_at (Pos hd)
-            >> simp[Once e_ce_rel_cases, Once ml_v_vals'_cases]
+            >> simp[Once e_ce_rel_cases, Once ml_v_vals_cases]
           )
           >> Cases_on ‘l'’ using SNOC_CASES
           >> gvs[vcons_list_def, LIST_REL_SNOC, REVERSE_SNOC]
@@ -2122,9 +2704,9 @@ Proof
             >> gvs[cps_transform_def, cps_app_ts_def]
             >> irule_at (Pos hd) EQ_REFL
             >> qpat_assum ‘cont_rel _ _’ $ irule_at (Pos hd)
-            >> qpat_assum ‘ml_v_vals' _ _’ $ irule_at Any
+            >> qpat_assum ‘ml_v_vals _ _’ $ irule_at Any
             >> simp[Once e_ce_rel_cases]
-            >> simp[Once ml_v_vals'_cases]
+            >> simp[Once ml_v_vals_cases]
             >> simp[cons_list_def]
             >> simp[scheme_env_def, env_rel_cases, FEVERY_FEMPTY]
           )
@@ -2272,7 +2854,7 @@ Theorem value_terminating:
     ⇒
     ∃ ck st' mlv . evaluate (st with clock:=ck) mlenv [mle]
       = (st', Rval [mlv]) ∧
-    ml_v_vals' v mlv ∧
+    ml_v_vals v mlv ∧
     st.ffi = st'.ffi
 Proof
   rpt strip_tac
